Definitions/Axioms.v
@@ -1,0 +1,72 @@
+From stdpp Require Import gmap.
+Require Import Definitions.DynamicActions.
+Require Import Definitions.Semantics.
+Require Import Definitions.Values.
+Require Import Definitions.GHeap.
+Require Import Definitions.Expressions.
+Require Import Definitions.Types.
+
+(* Use these as constructors inside "Inductive Phi" *)
+Axiom Phi_Seq_Nil_L : forall phi, Phi_Seq Phi_Nil phi = phi.
+Axiom Phi_Seq_Nil_R : forall phi, Phi_Seq phi Phi_Nil = phi.
+Axiom Phi_Par_Nil_R : forall phi, Phi_Par phi Phi_Nil = phi.
+Axiom Phi_Par_Nil_L : forall phi, Phi_Par Phi_Nil phi = phi.
+
+Axiom TcHeap_Extended:
+  forall hp hp' ef1 ea1 ef2 ea2 v1 v2 env rho 
+  	heap heap_mu1 heap_mu2 sttym sttya acts_mu1 acts_mu2,
+    (heap, env, rho, Mu_App ef1 ea1) ⇓ (heap_mu1, v1, acts_mu1) ->
+
+    (heap, env, rho, Mu_App ef2 ea2) ⇓ (heap_mu2, v2, acts_mu2) ->
+    (Phi_Par acts_mu1 acts_mu2, hp) ==>* (Phi_Nil, hp') ->
+    TcHeap (heap_mu1, sttym) ->
+    TcHeap (heap_mu2, sttya) ->
+    TcHeap (hp', Functional_Map_Union sttym sttya).
+
+Axiom ReadOnlyWalkSameHeap:
+  forall acts_mu1 acts_mu2 h same_h,
+    ReadOnlyPhi (Phi_Par acts_mu1 acts_mu2) ->
+    (Phi_Par acts_mu1 acts_mu2, h) ==>* (Phi_Nil, same_h) ->
+    h ≡@{Heap} same_h.
+
+Axiom Functional_Map_Union_find:
+  forall sttya sttyb (l : ST.key),
+    ST.find (elt:=tau) l (Functional_Map_Union sttya sttyb) = ST.find (elt:=tau) l sttya.
+
+Axiom subst_rho_eps_aux_1 :
+ forall rho rho' n x e e1 sa sa',
+   lc_type_eps e ->
+   lc_type_sa sa' ->
+   (fold_subst_eps rho e1) = (fold_subst_eps rho' (closing_rgn_in_eps n x e)) ->
+   fold_subst_sa rho sa = fold_subst_sa rho' (closing_rgn_in_sa n x sa') /\ e1 sa /\ e sa'.
+
+
+Axiom TcValExtended:
+  forall  stty1 stty2 v1 v2 rho ty1 ty2,
+    TcVal (stty1, v1, subst_rho rho ty1) ->
+    TcVal (stty2, v2, subst_rho rho ty2) ->
+    TcVal (Functional_Map_Union stty1 stty2, Pair (v1, v2), subst_rho rho (Ty2_Pair ty1 ty2)).
+  
+
+ (* both ec' and ee' and evaluated with the same context, but twice: inside Bs_Mu_App and BS_EffApp*)
+Axiom MuAppAndEffAppShareArgument:
+ forall h'' env rho ef env' rho' f x ec' ee' ea aheap v eff facts1 aacts1 bacts1, 
+   (forall fheap h' bacts facts v' aacts, 
+      (h'', env, rho, ef) ⇓ (fheap, Cls (env', rho', Mu f x ec' ee'), facts) ->
+      (fheap, env, rho, ea) ⇓ (aheap, v, aacts) ->
+      (aheap, update_rec_E (f, Cls (env', rho', Mu f x ec' ee')) (x, v) env', rho', ec') ⇓ (h', v', bacts) ->
+      (h'', env, rho, Mu_App ef ea) ⇓ (h', v', Phi_Seq (Phi_Seq facts aacts)bacts)) -> 
+   (* above is the definition of the type constructor BS_Mu_App *)
+   (h'', env, rho, Eff_App ef ea) ⇓ (h'', eff, Phi_Seq (Phi_Seq facts1 aacts1) bacts1) ->
+   (aheap, update_rec_E (f, Cls (env', rho', Mu f x ec' ee')) (x, v) env', rho', ee') ⇓ (h'', eff, bacts1). 
+
+(* Assuming that MuAppIncludesEffectShareArgument is a "specification", this prove the necessary goal *)
+Lemma EvaluationEffectFromEffApp:
+ forall h'' env rho ef env' rho' f x ec' ee' ea aheap v eff facts1 aacts1 bacts1,
+   (h'', env, rho, Eff_App ef ea) ⇓ (h'', eff, Phi_Seq (Phi_Seq facts1 aacts1) bacts1) ->
+   (aheap, update_rec_E (f, Cls (env', rho', Mu f x ec' ee')) (x, v) env', rho', ee') ⇓ (h'', eff, bacts1).
+Proof.
+  intros.
+  inversion H using MuAppAndEffAppShareArgument.
+  intros. econstructor; eauto.
+Qed. 
