Proofs/EffectFacts.v
@@ -1,0 +1,890 @@
+Require Import Coq.Program.Equality.
+Require Import Coq.Sets.Ensembles.
+Require Import Coq.Lists.List.
+
+Require Import Definitions.Axioms.
+Require Import Definitions.GHeap.
+Require Import Definitions.Keys.
+Require Import Definitions.ComputedActions.
+Require Import Definitions.DynamicActions.
+Require Import Definitions.StaticActions.
+Require Import Definitions.Regions.
+Require Import Definitions.Types.
+
+
+Lemma UnionEmptyWithEffIsEff:
+  forall eff,
+    Union_Theta (Some empty_set) eff = eff.
+Proof.
+  intro.
+  induction eff; simpl; [| reflexivity]. 
+  apply f_equal.
+  assert (set_union empty_set a = a).
+  - apply Extensionality_Ensembles.
+    unfold Same_set, Included; split; intros x H_; unfold In in *.
+    * destruct H_; [inversion H | assumption ].
+    * apply Union_intror. assumption.
+  - assumption.    
+Qed.
+
+
+Lemma PhiInThetaTop:
+  forall phi, phi ⋞ Theta_Top.
+Proof.  
+  induction phi; intros; econstructor; try assumption; apply DAT_Top.
+Qed.
+
+Lemma EmptyUnionisEmptySet :
+  forall acts a,
+    acts = Empty_set ComputedAction ->
+    a = Empty_set ComputedAction ->
+    Union ComputedAction acts a =  Empty_set ComputedAction.
+Proof.
+  intros acts a H1 H2.
+  apply Extensionality_Ensembles.
+  unfold Same_set, Included.
+  split.
+  - intros x Hx. rewrite H1 in Hx. 
+    replace (Union ComputedAction (Empty_set ComputedAction) a) 
+    with a in Hx 
+    by (apply Extensionality_Ensembles;
+        unfold Same_set, Included; split; intros y Hy; 
+        unfold In in *;
+          [apply Union_intror; assumption | destruct Hy; [inversion H | assumption]]).
+    rewrite H2 in Hx. inversion Hx.
+  - intros x Hx. inversion Hx.
+Qed. 
+
+Lemma EmptyUnionisEmptySet_2 :
+  forall acts a,
+    Union ComputedAction acts a =  Empty_set ComputedAction -> 
+    acts = Empty_set ComputedAction /\ a = Empty_set ComputedAction.
+Proof.
+  intros. split.
+  + rewrite <- H.
+    apply Extensionality_Ensembles.
+    unfold Same_set, Included.
+    split; intros. 
+    * apply Union_introl; assumption.
+    * rewrite H in H0. inversion H0.
+ + rewrite <- H.
+   apply Extensionality_Ensembles.
+   unfold Same_set, Included.
+   split; intros. 
+   * apply Union_intror; assumption.
+   * rewrite H in H0. inversion H0.
+Qed.
+
+Lemma EmptyIsNil:
+  forall phi, phi ⋞ Theta_Empty -> phi = Phi_Nil.
+Proof.
+  induction phi; intros.
+  - reflexivity. 
+  - unfold Theta_Empty, empty_set in H. 
+    dependent induction H; inversion H; subst; try (solve [inversion H2]).
+    + clear H2. clear H0. clear a. clear acts. 
+      dependent induction H; try (solve [inversion H]); intros.
+      * eapply IHDA_in_Theta; eauto. apply EmptyUnionisEmptySet_2 in x.
+        destruct x; subst. intuition.
+      * eapply IHDA_in_Theta; eauto. apply EmptyUnionisEmptySet_2 in x.
+         destruct x; subst. intuition.
+    + dependent induction H; try (solve [inversion H]).
+      * eapply IHDA_in_Theta; eauto.  apply EmptyUnionisEmptySet_2 in x.
+        destruct x; subst. intuition.
+      * eapply IHDA_in_Theta; eauto.  apply EmptyUnionisEmptySet_2 in x.
+        destruct x; subst. intuition.
+  - inversion H; subst. 
+    assert ( H_ : phi1 = Phi_Nil ) by (apply IHphi1; inversion H; assumption); rewrite H_.
+    assert ( H__ : phi2 = Phi_Nil ) by (apply IHphi2; inversion H; assumption); rewrite H__.
+    rewrite Phi_Par_Nil_R. reflexivity.
+  - assert ( H_ : phi1 = Phi_Nil ) by (apply IHphi1; inversion H; assumption); rewrite H_.
+    assert ( H__ : phi2 = Phi_Nil ) by (apply IHphi2; inversion H; assumption); rewrite H__.
+    rewrite Phi_Seq_Nil_R. reflexivity.
+Qed.
+
+
+Lemma EmptyInAnyTheta:
+  forall phi theta, phi ⋞ Theta_Empty -> phi ⋞ theta .
+Proof.  
+  induction phi; intros; try (solve [econstructor]).
+  - econstructor. unfold Theta_Empty, empty_set in H.
+    dependent induction H; dependent induction H; try (solve [inversion H]). 
+    * eapply IHDA_in_Theta; eauto. apply EmptyUnionisEmptySet_2 in x.
+        destruct x; subst. intuition.
+    * eapply IHDA_in_Theta; eauto. apply EmptyUnionisEmptySet_2 in x.
+        destruct x; subst. intuition.
+  - inversion H; subst.
+    apply PTS_Par; [ apply IHphi1; assumption | apply IHphi2; assumption]. 
+  - inversion H; subst.
+    apply PTS_Seq; [ apply IHphi1; assumption | apply IHphi2; assumption]. 
+Qed.
+
+Lemma EnsembleUnionSym:
+  forall (phi : Phi) (theta theta' : Theta),
+    phi ⋞ theta -> phi ⋞ (Union_Theta theta theta') /\ phi ⋞ (Union_Theta theta' theta).
+Proof.
+  intros phi theta theta' H.
+  generalize dependent theta'.
+  induction H; intros theta'.
+  - split; [apply PTS_Nil | apply PTS_Nil]. 
+  - destruct theta as [acts|]; destruct theta' as [acts'|]; 
+    intuition; simpl; try (solve [apply PTS_Elem; apply DAT_Top]). 
+    + apply PTS_Elem. apply DAT_intror. assumption.
+    + apply PTS_Elem. apply DAT_introl. assumption.    
+  - destruct theta as [acts|]; destruct theta' as [acts'|]; intuition;
+    (apply PTS_Seq; [apply IHPhi_Theta_Soundness1 | apply IHPhi_Theta_Soundness2]).
+  - split; destruct theta as [acts|]; destruct theta' as [acts'|]; intuition;
+    (apply PTS_Par; [apply IHPhi_Theta_Soundness1 | apply IHPhi_Theta_Soundness2]).  
+Qed.
+
+Lemma EmptyUnionIsIdentity : 
+  forall p eff, p ⋞ (Union_Theta (Some empty_set) eff) -> p ⋞ eff. 
+Proof.
+  intros p eff H; inversion H; subst; try apply PTS_Nil.  
+  induction eff; apply PTS_Elem;
+  try assert ( HUnionEmpty : (Union_Theta (Some empty_set)  (Some a)) = Some a) 
+    by (unfold Union_Theta, set_union, empty_set; f_equal;
+         apply Extensionality_Ensembles; red; split; unfold Included;
+         intros x Hx; [ inversion Hx; subst; [contradiction | assumption] | apply Union_intror]; auto).
+  -  rewrite HUnionEmpty in H0; assumption.
+  -   apply DAT_Top. 
+  - induction eff. assert ( HUnionEmpty : (Union_Theta (Some empty_set)  (Some a)) = Some a) 
+     by (unfold Union_Theta, set_union, empty_set; f_equal;
+         apply Extensionality_Ensembles; red; split; unfold Included;
+         intros x Hx; [ inversion Hx; subst; [contradiction | assumption] | apply Union_intror]; auto).
+    rewrite <- HUnionEmpty.  auto. now simpl in H.
+  -  induction eff. assert ( HUnionEmpty : (Union_Theta (Some empty_set)  (Some a)) = Some a) 
+     by (unfold Union_Theta, set_union, empty_set; f_equal;
+         apply Extensionality_Ensembles; red; split; unfold Included;
+         intros x Hx; [ inversion Hx; subst; [contradiction | assumption] | apply Union_intror]; auto).
+    rewrite <- HUnionEmpty. auto. now simpl in H. 
+Qed.
+
+Lemma EmptyUnionIsIdentity_2 : 
+  forall p eff,  p ⋞ eff -> p ⋞ (Union_Theta (Some empty_set) eff). 
+Proof.
+  intros p eff H; inversion H; subst; try apply PTS_Nil.  
+  induction eff; apply PTS_Elem;
+  try assert ( HUnionEmpty : (Union_Theta (Some empty_set)  (Some a)) = Some a) 
+      by (unfold Union_Theta, set_union, empty_set; f_equal;
+         apply Extensionality_Ensembles; red; split; unfold Included;
+         intros x Hx; [ inversion Hx; subst; [contradiction | assumption] | apply Union_intror]; auto).
+  - rewrite HUnionEmpty. assumption.
+  - apply DAT_Top.
+  - induction eff. 
+    assert ( HUnionEmpty : (Union_Theta (Some empty_set)  (Some a)) = Some a) 
+     by (unfold Union_Theta, set_union, empty_set; f_equal;
+         apply Extensionality_Ensembles; red; split; unfold Included;
+         intros x Hx; [ inversion Hx; subst; [contradiction | assumption] | apply Union_intror]; auto).
+    + rewrite HUnionEmpty. assumption.
+    + simpl. assumption.
+  - induction eff. 
+    assert ( HUnionEmpty : (Union_Theta (Some empty_set)  (Some a)) = Some a) 
+     by (unfold Union_Theta, set_union, empty_set; f_equal;
+         apply Extensionality_Ensembles; red; split; unfold Included;
+         intros x Hx; [ inversion Hx; subst; [contradiction | assumption] | apply Union_intror]; auto).
+    + rewrite HUnionEmpty. assumption.
+    + simpl. assumption.  
+Qed.
+
+Lemma EnsembleUnionComp :
+  forall (phi1 phi2 : Phi) (theta1 theta2 : Theta),
+    phi1 ⋞ theta1 -> phi2 ⋞ theta2 -> Phi_Seq phi1  phi2 ⋞ (Union_Theta theta1 theta2).
+Proof. 
+  intros phi1 phi2 theta1 theta2 H1 H2.
+  econstructor.
+  - apply EnsembleUnionSym with (theta' := theta2) in H1. intuition. 
+  - apply EnsembleUnionSym with (theta' := theta1) in H2. intuition.
+Qed.
+
+
+Lemma Theta_introl: 
+  forall phi theta1 theta2, phi ⋞ theta1 -> phi ⋞ Union_Theta theta1 theta2.
+Proof.
+  induction phi; intros; try (solve [econstructor]).
+  - inversion H; subst; inversion H1; subst; simpl;
+    try (solve [assumption |
+                induction theta2; [econstructor; constructor; now apply Union_introl | econstructor; constructor] |
+                induction theta2; [econstructor; now apply DAT_intror | econstructor; constructor ]] ).
+  - apply PTS_Par. apply IHphi1. now inversion H. apply IHphi2. now inversion H.
+  - apply PTS_Seq. apply IHphi1. now inversion H. apply IHphi2. now inversion H.
+Qed.    
+
+Lemma Theta_intror:
+  forall phi theta1 theta2, phi ⋞ theta1 -> phi ⋞ Union_Theta theta2 theta1.
+Proof.
+  induction phi; intros; try (solve [econstructor]).
+  - inversion H; subst; inversion H1; subst; simpl;
+    try (solve [assumption |
+                induction theta2; [econstructor; constructor; now apply Union_intror | econstructor; constructor] |
+                induction theta2; [econstructor; now apply DAT_introl | econstructor; constructor ]] ).
+  - apply PTS_Par. apply IHphi1. now inversion H. apply IHphi2. now inversion H.
+  - apply PTS_Seq. apply IHphi1. now inversion H. apply IHphi2. now inversion H.
+Qed.
+
+
+Lemma Disjointness_app_or_r :
+  forall phi1 phi2 phi3,
+    Disjoint_Traces (phi_as_list phi1 ++ phi_as_list phi2) (phi_as_list phi3) ->
+    Disjoint_Traces (phi_as_list phi1) (phi_as_list phi3) \/
+    Disjoint_Traces (phi_as_list phi2) (phi_as_list phi3).
+Proof.
+  intros phi1 phi2 phi3 H. 
+  dependent induction H.
+  left; econstructor; intros.
+  apply H;  [ apply in_or_app; left | ]; assumption.
+Qed.
+
+Lemma Disjointness_app_or_l :
+  forall phi1 phi2 phi3,
+    Disjoint_Traces (phi_as_list phi1) (phi_as_list phi2 ++ phi_as_list phi3) ->
+    Disjoint_Traces (phi_as_list phi1) (phi_as_list phi2) \/
+    Disjoint_Traces (phi_as_list phi1) (phi_as_list phi3).
+Proof.
+  intros phi1 phi2 phi3 H. 
+  dependent induction H.
+  left; econstructor; intros.
+  apply H;  [ | apply in_or_app; left]; assumption.
+Qed.
+
+Lemma Disjointness_app_app_and_r :
+  forall phi1 phi2 phi3,
+    Disjoint_Traces (phi_as_list phi1 ++ phi_as_list phi2) (phi_as_list phi3) ->
+    Disjoint_Traces (phi_as_list phi1) (phi_as_list phi3) /\
+    Disjoint_Traces (phi_as_list phi2) (phi_as_list phi3).
+Proof.
+  intros phi1 phi2 phi3 H.  
+  dependent induction H; split.
+  - econstructor; intros. apply H;  [ apply in_or_app; left | ]; assumption.
+  - econstructor; intros. apply H;  [ apply in_or_app; right | ]; assumption.
+Qed.
+
+Lemma Disjointness_app_app_and_l :
+  forall phi1 phi2 phi3,
+    Disjoint_Traces (phi_as_list phi1) (phi_as_list phi2 ++ phi_as_list phi3) ->
+    Disjoint_Traces (phi_as_list phi1) (phi_as_list phi2) /\
+    Disjoint_Traces (phi_as_list phi1) (phi_as_list phi3).
+Proof.
+  intros phi1 phi2 phi3 H.  
+  dependent induction H; split.
+  - econstructor; intros. apply H; [ |  apply in_or_app; left ]; assumption.
+  - econstructor; intros. apply H;  [ | apply in_or_app; right ]; assumption.
+Qed.
+
+Lemma Disjointness_and_app_r :
+  forall phi1 phi2 phi3,
+    Disjoint_Traces (phi_as_list phi1) (phi_as_list phi3) /\
+    Disjoint_Traces (phi_as_list phi2) (phi_as_list phi3) ->
+    Disjoint_Traces (phi_as_list phi1 ++ phi_as_list phi2) (phi_as_list phi3).
+Proof.
+  intros phi1 phi2 phi3 H. destruct H. 
+  generalize dependent phi2.
+  dependent induction H; intros.
+  econstructor; intros.
+  rename H into H1_3. inversion H0 as [? ? H2_3]; subst.
+  apply in_app_or in H1; destruct H1; [apply H1_3 | apply H2_3]; auto.
+Qed.
+
+Lemma Disjointness_and_app_l :
+  forall phi1 phi2 phi3,
+    Disjoint_Traces (phi_as_list phi1) (phi_as_list phi2) /\
+    Disjoint_Traces (phi_as_list phi1) (phi_as_list phi3) ->
+    Disjoint_Traces (phi_as_list phi1) (phi_as_list phi2 ++ phi_as_list phi3).
+Proof.
+  intros phi1 phi2 phi3 H. destruct H. 
+  generalize dependent phi2.
+  dependent induction H0; intros.
+  econstructor; intros. 
+  rename H into H1_3. inversion H0 as [? ? H1_2]; subst.
+  apply in_app_or in H2; destruct H2; [apply H1_2 | apply H1_3]; auto.
+Qed.
+
+Lemma Conflictness_app_or_l :
+  forall phi1 phi2 phi3,
+    Det_Trace phi1 ->
+    Det_Trace phi2 ->
+    Det_Trace phi3 ->
+    ~ Conflict_Traces (phi_as_list phi1) (phi_as_list phi2 ++ phi_as_list phi3) ->
+    ~ Conflict_Traces (phi_as_list phi1) (phi_as_list phi2) \/
+    ~ Conflict_Traces (phi_as_list phi1) (phi_as_list phi3). 
+Proof.
+  intros phi1 phi2 phi3 HDet1 HDet2 HDet3 H. unfold not in *.
+  left. intro. apply H. clear H.  
+  dependent induction H0;
+    inversion HDet1; inversion HDet2; inversion HDet3; subst; simpl in *;
+    try (solve [contradiction |
+                intuition; subst; econstructor; eauto; apply in_eq |
+                intuition; subst; inversion HDet3; subst; econstructor; eauto; apply in_eq |
+                intuition; subst; rewrite app_nil_r; econstructor; eauto; apply in_eq |
+                intuition; subst; econstructor; eauto; [apply in_eq | apply in_or_app; left; assumption] |
+                 econstructor; eauto;  apply in_or_app; left; assumption
+               ]).
+Qed.
+
+Lemma Conflictness_app_or_r :
+  forall phi1 phi2 phi3,
+    Det_Trace phi1 ->
+    Det_Trace phi2 ->
+    Det_Trace phi3 ->
+    ~ Conflict_Traces (phi_as_list phi1 ++ phi_as_list phi2) (phi_as_list phi3) ->
+    ~ Conflict_Traces (phi_as_list phi1) (phi_as_list phi3) \/
+    ~ Conflict_Traces (phi_as_list phi2) (phi_as_list phi3). 
+Proof.
+  intros phi1 phi2 phi3 HDet1 HDet2 HDet3 H. unfold not in *.
+  left. intro. apply H. clear H.  
+  dependent induction H0;
+    inversion HDet1; inversion HDet2; inversion HDet3; subst; simpl in *;
+    try (solve [contradiction |
+                intuition; subst; econstructor; [ apply in_eq | apply in_eq | eassumption] |
+                intuition; subst; econstructor; [ apply in_eq | eassumption | assumption] |
+                intuition; subst; econstructor; [rewrite app_nil_r; eassumption |  apply in_eq | assumption ] |
+                intuition; subst; econstructor; [rewrite app_nil_r; eassumption | eassumption | assumption ] |
+                intuition; subst; econstructor; [apply in_or_app; left; eassumption |  apply in_eq | assumption ] |
+                intuition; subst; econstructor; [ apply in_or_app; left; eassumption | eassumption | assumption ]
+               ]).
+Qed.
+
+Lemma Conflictness_app_and_l :
+  forall phi1 phi2 phi3,
+    Det_Trace phi1 ->
+    Det_Trace phi2 ->
+    Det_Trace phi3 ->
+    ~ Conflict_Traces (phi_as_list phi1) (phi_as_list phi2 ++ phi_as_list phi3) ->
+    ~ Conflict_Traces (phi_as_list phi1) (phi_as_list phi2) /\
+    ~ Conflict_Traces (phi_as_list phi1) (phi_as_list phi3). 
+Proof.
+  intros phi1 phi2 phi3 HDet1 HDet2 HDet3 H. unfold not in *.
+  split.
+  - intro. apply H. clear H.
+    dependent induction H0;
+      inversion HDet1; inversion HDet2; inversion HDet3; subst; simpl in *;
+      try (solve [contradiction |
+                intuition; subst; econstructor; eauto; apply in_eq |
+                intuition; subst; inversion HDet3; subst; econstructor; eauto; apply in_eq |
+                intuition; subst; rewrite app_nil_r; econstructor; eauto; apply in_eq |
+                intuition; subst; econstructor; eauto; [apply in_eq | apply in_or_app; left; assumption] |
+                 econstructor; eauto;  apply in_or_app; left; assumption
+                 ]).
+  -  intro. apply H. clear H.
+    dependent induction H0;
+      inversion HDet1; inversion HDet2; inversion HDet3; subst; simpl in *;
+      try (solve [contradiction |
+                  econstructor; eauto;  apply in_or_app; right; assumption |
+                  intuition; subst; econstructor; eauto; [ apply in_eq | apply in_cons; apply in_eq] |
+                  intuition; subst; econstructor; eauto; [ apply in_eq | apply in_cons; assumption] |
+                  intuition; subst; econstructor; eauto; apply in_cons; apply in_eq |
+                  intuition; subst; econstructor; eauto; apply in_cons;assumption
+                 ]).
+Qed.
+
+
+Lemma Conflictness_app_and_r :
+  forall phi1 phi2 phi3,
+    Det_Trace phi1 ->
+    Det_Trace phi2 ->
+    Det_Trace phi3 ->
+    ~ Conflict_Traces (phi_as_list phi1 ++ phi_as_list phi2) (phi_as_list phi3) ->
+    ~ Conflict_Traces (phi_as_list phi1) (phi_as_list phi3) /\
+    ~ Conflict_Traces (phi_as_list phi2) (phi_as_list phi3). 
+Proof.
+  intros phi1 phi2 phi3 HDet1 HDet2 HDet3 H. unfold not in *.
+  split.
+  - intro. apply H. clear H.
+    dependent induction H0;
+      inversion HDet1; inversion HDet2; inversion HDet3; subst; simpl in *;
+      try (solve [contradiction |
+                intuition; subst; econstructor; eauto; apply in_eq |
+                intuition; subst; inversion HDet3; subst; econstructor; eauto; apply in_eq |
+                intuition; subst; rewrite app_nil_r; econstructor; eauto; apply in_eq |
+                intuition; subst; econstructor; eauto; [apply in_eq | apply in_or_app; left; assumption] |
+                 econstructor; eauto;  apply in_or_app; left; assumption
+                 ]).
+  -  intro. apply H. clear H.
+    dependent induction H0;
+      inversion HDet1; inversion HDet2; inversion HDet3; subst; simpl in *;
+      try (solve [contradiction |
+                  econstructor; eauto;  apply in_or_app; right; assumption |
+                  intuition; subst; econstructor; eauto; [ apply in_eq | apply in_cons; apply in_eq] |
+                  intuition; subst; econstructor; eauto; apply in_cons; apply in_eq |
+                  intuition; subst; econstructor; eauto; apply in_cons;assumption |
+                  intuition; subst; econstructor; eauto; [apply in_cons; apply in_eq | apply in_eq] |
+                  intuition; subst; econstructor; eauto; [apply in_cons; assumption | apply in_eq]
+                 ]).
+Qed.
+
+Lemma Conflictness_or_app_l :
+  forall phi1 phi2 phi3,
+    Conflict_Traces (phi_as_list phi1) (phi_as_list phi2) \/
+    Conflict_Traces (phi_as_list phi1) (phi_as_list phi3) ->
+    Conflict_Traces (phi_as_list phi1) (phi_as_list phi2 ++ phi_as_list phi3).
+Proof.
+  intros phi1 phi2 phi3 H.
+  destruct H. 
+  - dependent induction H. econstructor; eauto. apply in_or_app. left; assumption.
+  - dependent induction H. econstructor; eauto. apply in_or_app. right; assumption.
+Qed.
+
+Lemma Conflictness_or_app_r :
+  forall phi1 phi2 phi3,
+    Conflict_Traces (phi_as_list phi1) (phi_as_list phi3) \/
+    Conflict_Traces (phi_as_list phi2) (phi_as_list phi3) ->
+    Conflict_Traces (phi_as_list phi1 ++ phi_as_list phi2) (phi_as_list phi3).
+Proof.
+  intros phi1 phi2 phi3 H.
+  destruct H. 
+  - dependent induction H. econstructor; eauto. apply in_or_app. left; assumption.
+  - dependent induction H. econstructor; eauto. apply in_or_app. right; assumption.
+Qed.
+ 
+Lemma Conflictness_and_app_l :
+  forall phi1 phi2 phi3,
+    ~ Conflict_Traces (phi_as_list phi1 ) (phi_as_list phi2 ) /\
+    ~ Conflict_Traces (phi_as_list phi1 ) (phi_as_list phi3 ) ->
+    ~ Conflict_Traces (phi_as_list phi1 ) (phi_as_list phi2  ++ phi_as_list phi3 ).
+Proof.
+  intros phi1 phi2 phi3 H. unfold not in *. destruct H. 
+  intro. dependent induction H1.  apply in_app_or in H3. intuition.
+  + apply H. econstructor; eauto.
+  + apply H0. econstructor; eauto. 
+Qed.
+
+
+Lemma Conflictness_and_app_r :
+  forall phi1 phi2 phi3,
+    ~ Conflict_Traces (phi_as_list phi1 ) (phi_as_list phi3 ) /\
+    ~ Conflict_Traces (phi_as_list phi2 ) (phi_as_list phi3 ) ->
+    ~ Conflict_Traces (phi_as_list phi1 ++ phi_as_list phi2)  (phi_as_list phi3 ).
+Proof.
+  intros phi1 phi2 phi3 H. unfold not in *. destruct H. 
+  intro. dependent induction H1.  apply in_app_or in H3. intuition.
+  + apply H. econstructor; eauto.
+  + apply H0. econstructor; eauto. 
+Qed.
+
+
+
+Inductive SA_DA_Soundness : StaticAction -> DynamicAction -> Prop :=
+| SA_DA_Read : forall r l v, SA_DA_Soundness (SA_Read (Rgn2_Const true true r)) (DA_Read r l v)
+| SA_DA_Write : forall r l v, SA_DA_Soundness (SA_Write (Rgn2_Const true true r)) (DA_Write r l v)
+| SA_DA_Alloc : forall r l v, SA_DA_Soundness (SA_Alloc (Rgn2_Const true true r)) (DA_Alloc r l v).
+
+Inductive Epsilon_Phi_Soundness :  (Epsilon * Phi) -> Prop := 
+  | EPS : forall st dy, (forall da, DA_in_Phi da dy -> exists sa, Ensembles.In StaticAction st sa /\ SA_DA_Soundness sa da) -> Epsilon_Phi_Soundness (st, dy).
+
+Lemma ReadOnlyStaticImpliesReadOnlySubstStatic : 
+  forall eps rho,
+    ReadOnlyStatic eps ->
+    ReadOnlyStatic (fold_subst_eps rho eps).
+Proof.
+  intros eps rho ROS.
+  induction ROS.
+  - replace (fold_subst_eps rho Empty_Static_Action) with (Empty_Static_Action).
+    constructor.
+    apply Extensionality_Ensembles;
+    unfold Same_set, Included; split; intros x H; unfold Ensembles.In in *.
+    inversion H. inversion H. destruct H0. inversion H0.
+  - replace (fold_subst_eps rho (Singleton_Static_Action (SA_Read r))) with (Singleton_Static_Action (SA_Read (fold_subst_rgn rho r))).
+    constructor.
+    apply Extensionality_Ensembles;
+    unfold Same_set, Included; split; intros x H; unfold Ensembles.In in *.
+    inversion H.
+    unfold fold_subst_eps. exists (SA_Read r).
+    + split; [constructor | subst; simpl; reflexivity].
+    + inversion H. inversion H0. inversion H1. subst. unfold fold_subst_sa; simpl. apply Ensembles.In_singleton.
+  - replace (fold_subst_eps rho (Union_Static_Action eps1 eps2)) with (Union_Static_Action (fold_subst_eps rho eps1) (fold_subst_eps rho eps2)).
+    constructor; assumption.
+    apply Extensionality_Ensembles;
+    unfold Same_set, Included; split; intros x H; unfold Ensembles.In in *.
+    + inversion H; subst; inversion H0; unfold fold_subst_eps; exists x0; split.
+      * apply Ensembles.Union_introl. destruct H1; subst. assumption.
+      * destruct H1; subst. reflexivity. 
+      * apply Ensembles.Union_intror. destruct H1; subst. assumption.
+      * destruct H1; subst. reflexivity.   
+   + inversion H. inversion H0. inversion H1; subst;
+       [apply Ensembles.Union_introl | apply Ensembles.Union_intror];
+       unfold Ensembles.In; unfold fold_subst_eps; exists x0.
+     * split; [assumption | reflexivity].
+     * split; [assumption | reflexivity].
+Qed.
+
+Lemma ReadOnlyStaticImpliesReadOnlyPhi :
+  forall eps phi,
+    ReadOnlyStatic eps ->
+    Epsilon_Phi_Soundness (eps, phi) ->
+    ReadOnlyPhi phi.
+Proof.
+  intros eps phi. induction phi; intros ROS H.
+  - constructor.
+  - induction d.
+    + exfalso; induction ROS.
+      * inversion H; subst. 
+        edestruct H1; [econstructor | destruct H0 ; inversion H0].
+      * inversion H; subst.
+        edestruct H1; [econstructor | destruct H0 ; inversion H0; subst; inversion H2 ].
+      * inversion H; subst. destruct (H1 (DA_Alloc r n v)) as [ ? [ ? ? ]]; [ constructor | ].
+        inversion H0; subst.
+        apply IHROS1; constructor; intros; inversion H4; subst; exists x; intuition.
+        apply IHROS2; constructor; intros; inversion H4; subst; exists x; intuition.
+    + econstructor.
+    + exfalso; induction ROS.
+      * inversion H; subst. 
+        edestruct H1; [econstructor | destruct H0 ; inversion H0].
+      * inversion H; subst.
+        edestruct H1; [econstructor | destruct H0 ; inversion H0; subst; inversion H2 ].
+      * inversion H; subst. destruct (H1 (DA_Write r n v)) as [ ? [ ? ? ]]; [ constructor | ].
+        inversion H0; subst.
+        apply IHROS1; constructor; intros; inversion H4; subst; exists x; intuition.
+        apply IHROS2; constructor; intros; inversion H4; subst; exists x; intuition.
+  - assert (Epsilon_Phi_Soundness (eps, phi1)).
+    constructor; intros da daIn; inversion H; subst; apply (H1 da); apply DAP_Par; auto.
+    assert (Epsilon_Phi_Soundness (eps, phi2)).
+    constructor; intros da daIn; inversion H; subst; apply (H2 da); apply DAP_Par; auto.
+    constructor; auto.
+  - assert (Epsilon_Phi_Soundness (eps, phi1)).
+    constructor; intros da daIn; inversion H; subst; apply (H1 da); apply DAP_Seq; auto.
+    assert (Epsilon_Phi_Soundness (eps, phi2)).
+    constructor; intros da daIn; inversion H; subst; apply (H2 da); apply DAP_Seq; auto.
+    constructor; auto.
+Qed.
+
+
+Lemma EmptyUnionisEmptySet_Name_Left :
+  forall acts,
+    Union VarId (Empty_set VarId) acts = acts.
+Proof.
+  intros acts;
+  apply Extensionality_Ensembles;
+  unfold Same_set, Included;
+  split.
+  - intros x Hx. unfold In in *. destruct Hx; auto. inversion H.
+  - intros x Hx. apply Union_intror. assumption.
+Qed. 
+
+Lemma EmptyUnionisEmptySet_Name_Right :
+  forall acts,
+    Union VarId acts (Empty_set VarId) = acts.
+Proof.
+  intros acts;
+  apply Extensionality_Ensembles;
+  unfold Same_set, Included;
+  split.
+  - intros x Hx. unfold In in *. destruct Hx; auto. inversion H.
+  - intros x Hx. apply Union_introl. assumption.
+Qed. 
+
+Lemma IncludedRemoveSingleton:
+  forall n x rgns,
+    n <> x ->
+    included (singleton_set n) (Union VarId rgns (singleton_set x)) ->
+    included (singleton_set n) rgns.
+Proof.
+  intros n x rgns H1 H2.
+  unfold included, Included, In in *. 
+  intro. intro.  destruct (H2 x0); auto.  
+  inversion H; subst. 
+  contradict H0. intro. inversion H0. 
+  apply H1. symmetry. assumption.
+Qed.
+
+Lemma IncludedUnion_Name_1:
+  forall (a b : Ensemble VarId) rgns,
+    included (set_union a b) rgns ->
+    included a rgns /\
+    included b rgns.
+Proof.
+  intros.
+  split.
+  - intro. intro. apply H.
+    apply Union_introl. assumption.
+  - intro. intro. apply H.
+    + apply Union_intror. assumption.
+Qed.
+
+Lemma IncludedUnion_Name_5:
+  forall (a b c : Ensemble VarId) rgns,
+    included (set_union a b)
+             (set_union rgns c) ->
+    included a (set_union rgns c) /\
+    included b (set_union rgns c).
+Proof.
+  intros.
+  split.
+  - intro. intro. apply H.
+    apply Union_introl. assumption.
+  - intro. intro. apply H.
+    apply Union_intror. assumption.    
+Qed.
+
+Lemma IncludedUnion_Name_4:
+  forall (a b c : Ensemble VarId) rgns,
+    included (set_union a b) rgns /\
+    included (set_union a c) rgns ->
+    included (set_union a (set_union c b)) rgns.
+Proof.
+  intros. 
+  intro. intro. unfold In, set_union in *.
+  destruct H.
+  apply IncludedUnion_Name_1 in H. destruct H.
+  apply IncludedUnion_Name_1 in H1. destruct H1.
+  repeat destruct H0; [apply H1 | apply H3 | apply H2]; assumption. 
+Qed.
+
+Lemma IncludedUnion_Static_Action_4:
+  forall (a b : Ensemble StaticAction) (rgns : Ensemble VarId) (x : VarId),
+    (free_rgn_vars_in_eps a x -> rgns x) ->
+    (free_rgn_vars_in_eps b x -> rgns x) ->                        
+    (free_rgn_vars_in_eps (Union_Static_Action a b) x -> rgns x).
+Proof.
+  intros a b rgns x H1 H2 H3.
+  unfold free_rgn_vars_in_eps in *.
+  destruct H3 as [sa [H4 H5]].
+  destruct H4; [apply H1 | apply H2]; exists x0; auto.
+Qed.
+
+Lemma IncludedUnion_Name_6:
+  forall (a b: Ensemble VarId) rgns,
+    included a rgns /\
+    included b rgns ->
+    included (set_union a b) rgns.
+Proof.
+  intros. 
+  intro. intro. unfold In, set_union in *.
+  destruct H0; destruct H; [apply H | apply H1]; assumption. 
+Qed.
+
+Lemma RegionAbsFrv_2:
+  forall  x r rgns n,
+    included (free_rgn_vars_in_rgn r) (set_union rgns (singleton_set x)) ->
+    included (free_rgn_vars_in_rgn (closing_rgn_in_rgn n x r)) rgns.
+Proof.
+  intros. unfold Region_in_Type in r. 
+  dependent induction r; simpl in *; do 2 intro.
+  - inversion H0.
+  - destruct (RMapProp.F.eq_dec v x); subst.
+    + simpl in *. inversion H0.
+    + apply IncludedRemoveSingleton in H; auto.
+  - inversion H0.
+Qed. 
+
+
+
+Lemma NoFreeVarsAfterClosingRgn:
+  forall n x r,
+    ~ free_rgn_vars_in_rgn (closing_rgn_in_rgn n x r) x.
+Proof.
+  intros n x r.
+  unfold Region_in_Type in r. dependent induction r; intro;
+  unfold free_rgn_vars_in_rgn, closing_rgn_in_rgn in H.
+  - inversion H.
+  - destruct (RMapProp.F.eq_dec v x); subst.
+    + inversion H.
+    + inversion H. apply n0. assumption.
+  - inversion H.
+Qed.
+
+Lemma NoFreeVarsAfterClosingSa:
+ forall n sa x,
+   ~ free_rgn_vars_in_sa (closing_rgn_in_sa n x sa) x.
+Proof.
+  intros n sa x. intro.
+  induction sa;
+  unfold free_rgn_vars_in_sa, closing_rgn_in_sa in H; 
+  eapply NoFreeVarsAfterClosingRgn; eauto.
+Qed.
+
+
+
+
+Lemma RegionAbsFrv_1:
+   forall effr rgns (x : VarId) n, 
+     included (free_rgn_vars_in_eps effr) (set_union rgns (singleton_set x)) ->
+     included (free_rgn_vars_in_eps (closing_rgn_in_eps n x effr)) rgns.
+Proof.
+  intros effr rgns x n H.
+  unfold free_rgn_vars_in_eps in *.
+  do 2 intro. unfold In in *.
+  destruct H0 as [sa [H1 H2]].
+  unfold closing_rgn_in_eps in H1.
+  destruct H1 as [sa' [H3 H4]].
+  rewrite <- H4 in H2. 
+  unfold included, Included, In in H.
+  destruct (H x0); auto.
+  - exists sa'. intuition.
+    destruct (RMapProp.F.eq_dec x x0); subst.
+    + contradict H2. apply NoFreeVarsAfterClosingSa.
+    + induction sa'; unfold Region_in_Type in r; dependent induction r; 
+      simpl in *; unfold free_rgn_vars_in_rgn in *;
+      try (solve [inversion H2 | destruct  (RMapProp.F.eq_dec v x); subst; [inversion H2 | assumption]]).
+  - destruct (RMapProp.F.eq_dec x x0); subst.
+    + contradict H2. apply NoFreeVarsAfterClosingSa.
+    + exfalso. contradict n0. inversion H0. auto.
+Qed.
+
+Lemma RegionAbsFrv_3:
+   forall tyr rgns (x : VarId), 
+     included (frv tyr) (set_union rgns (singleton_set x)) ->
+     included (frv (close_var x tyr)) rgns. 
+Proof.
+  intros tyr rgns x H.
+  unfold close_var.
+  generalize 0.
+  dependent induction tyr; simpl in *; intro;
+  try (solve [intro; intro; inversion H0]).
+  - unfold included, Included, In in *. 
+    intro. intro.  
+    destruct H0.
+    + eapply IHtyr1; auto. 
+      intro. intro. apply H.
+      apply Union_introl. assumption. eassumption.
+    + eapply IHtyr2; auto.
+      intro. intro. apply H.
+      apply Union_intror. assumption. eassumption.
+  - apply IncludedUnion_Name_6.
+    split.
+    + apply IncludedUnion_Name_1 in H. destruct H. clear H0. 
+      apply RegionAbsFrv_2; eauto.
+    + eapply IHtyr.
+      do 2 intro. apply H.
+       apply Union_intror. assumption.
+  - repeat (apply IncludedUnion_Name_4; split); 
+    apply IncludedUnion_Name_6; split;
+    try (solve [apply IHtyr1; do 2 intro; apply H; apply Union_introl; assumption]).
+    + apply IHtyr3. intro. intro.
+      apply H.
+      apply Union_intror. apply Union_intror. apply Union_intror. assumption. 
+    + apply IHtyr2. intro. intro.
+      apply H.
+      apply Union_intror. apply Union_intror. apply Union_introl. assumption. 
+    + apply IncludedUnion_Name_5 in H; destruct H as [H1  H]. clear H1.
+      apply IncludedUnion_Name_5 in H; destruct H as [H  H1]. clear H1.
+      apply IncludedUnion_Name_5 in H; destruct H as [H1  H]. clear H1.
+      eapply RegionAbsFrv_1; eauto.
+    + apply IncludedUnion_Name_5 in H; destruct H as [H1  H]. clear H1.
+      apply IncludedUnion_Name_5 in H; destruct H as [H  H1]. clear H1.
+      apply IncludedUnion_Name_5 in H; destruct H as [H  H1]. clear H1.
+      eapply RegionAbsFrv_1; eauto.
+  - apply IncludedUnion_Name_6.
+    split.
+    + apply IncludedUnion_Name_1 in H. destruct H. clear H0.
+      eapply RegionAbsFrv_1; eauto.
+    + apply IHtyr.
+      do 2 intro.
+      apply H. apply Union_intror. assumption. 
+Qed.  
+
+Lemma RegionAppFrv_2:
+  forall region r x n,
+    lc_type_rgn r ->
+    free_rgn_vars_in_rgn (opening_rgn_in_rgn n region r) x ->
+    free_rgn_vars_in_rgn r x.
+Proof.
+  intros.
+  unfold Region_in_Type in r.
+  dependent induction r; simpl in *.
+  - inversion H0.
+  - assumption.
+  - inversion H.
+Qed.
+
+Lemma RegionAppFrv_3:
+  forall region e x n,
+    lc_type_eps e ->
+    free_rgn_vars_in_eps (opening_rgn_in_eps n region e) x ->
+    free_rgn_vars_in_eps e x.
+Proof.
+  intros region e x n H1 H2.
+  inversion H1; subst.
+  unfold free_rgn_vars_in_eps in *.
+  destruct H2 as [sa [H3 H4]].
+  destruct (H sa).
+  exists sa. auto.
+Qed.
+
+Lemma RegionAppFrv_1:
+  forall tyr rgns w,
+    lc_type tyr ->
+    included (frv tyr) rgns ->
+    included (frv (open (mk_rgn_type w) tyr)) rgns.
+Proof.
+  intros tyr rgns w Hlc H.
+  unfold open.
+  generalize 0.
+  unfold Region_in_Expr in w; intro.
+  dependent induction w; simpl.
+  - dependent induction tyr; simpl in *;
+    inversion Hlc; subst;
+    try (solve [do 2 intro; inversion H | do 2 intro; inversion H0]).
+    + apply IncludedUnion_Name_6.
+      split; [apply IHtyr1 |  apply IHtyr2]; auto.
+      * do 2 intro. apply H; simpl.
+        apply Union_introl. assumption.
+      * do 2 intro. apply H; simpl.
+        apply Union_intror. assumption. 
+    + apply IncludedUnion_Name_6.
+      split.
+      * do 2 intro. apply H; simpl.
+        apply Union_introl. unfold In in *. 
+        eapply RegionAppFrv_2; eauto.
+      * apply IHtyr; auto. do 2 intro. 
+        apply H; simpl.
+        apply Union_intror. assumption. 
+    + apply IncludedUnion_Name_6. 
+      split; [apply IHtyr1; auto; do 2 intro; apply H; simpl; apply Union_introl; assumption |].
+      apply IncludedUnion_Name_6.
+      split; [apply IncludedUnion_Name_6; split | apply IncludedUnion_Name_6; split].
+      * do 2 intro. apply H; simpl. 
+        apply Union_intror. apply Union_introl. apply Union_introl.
+        unfold In in *.
+        eapply RegionAppFrv_3; eauto.
+      * do 2 intro. apply H; simpl. 
+        apply Union_intror. apply Union_introl. apply Union_intror.
+        unfold In in *.
+        eapply RegionAppFrv_3; eauto.
+      * apply IHtyr2; auto; do 2 intro; apply H; simpl. 
+        apply Union_intror; apply Union_intror. apply Union_introl. assumption.
+      * apply IHtyr3; auto; do 2 intro; apply H; simpl. 
+        apply Union_intror; apply Union_intror. apply Union_intror. assumption.
+    + apply IncludedUnion_Name_6. 
+      split; [| apply IHtyr; auto; do 2 intro; apply H; simpl; apply Union_intror; assumption].
+      do 2 intro. apply H; simpl in *.
+      apply Union_introl.  unfold In in *.
+      eapply RegionAppFrv_3; eauto.
+  - dependent induction tyr; simpl;
+    inversion Hlc; subst;
+    try (solve [do 2 intro; inversion H0]).
+    + apply IncludedUnion_Name_6.
+      split; [apply IHtyr1 |  apply IHtyr2]; auto.
+      * do 2 intro. apply H; simpl.
+        apply Union_introl. assumption.
+      * do 2 intro. apply H; simpl.
+        apply Union_intror. assumption. 
+    + apply IncludedUnion_Name_6.
+      split.
+      * do 2 intro. apply H; simpl.
+        apply Union_introl. unfold In in *. 
+        eapply RegionAppFrv_2; eauto.
+      * apply IHtyr; auto. do 2 intro. 
+        apply H; simpl.
+        apply Union_intror. assumption. 
+    + apply IncludedUnion_Name_6. 
+      split; [apply IHtyr1; auto; do 2 intro; apply H; simpl; apply Union_introl; assumption |].
+      apply IncludedUnion_Name_6.
+      split; [apply IncludedUnion_Name_6; split | apply IncludedUnion_Name_6; split].
+      * do 2 intro. apply H; simpl. 
+        apply Union_intror. apply Union_introl. apply Union_introl.
+        unfold In in *.
+        eapply RegionAppFrv_3; eauto.
+      * do 2 intro. apply H; simpl. 
+        apply Union_intror. apply Union_introl. apply Union_intror.
+        unfold In in *.
+        eapply RegionAppFrv_3; eauto.
+      * apply IHtyr2; auto; do 2 intro; apply H; simpl. 
+        apply Union_intror; apply Union_intror. apply Union_introl. assumption.
+      * apply IHtyr3; auto; do 2 intro; apply H; simpl. 
+        apply Union_intror; apply Union_intror. apply Union_intror. assumption.
+    + apply IncludedUnion_Name_6. 
+      split; [| apply IHtyr; auto; do 2 intro; apply H; simpl; apply Union_intror; assumption].
+      do 2 intro. apply H; simpl in *.
+      apply Union_introl.  unfold In in *.
+      eapply RegionAppFrv_3; eauto.
+Qed.
