Proofs/HeapFacts.v
@@ -1,0 +1,488 @@
+From stdpp Require Import gmap.
+Require Import Coq.Program.Equality.
+Require Import Definitions.GHeap.
+Require Import Definitions.Types.
+Require Import Definitions.Values.
+Require Import Definitions.Semantics.
+Require Import Definitions.DynamicActions.
+Require Import Proofs.TypeFacts.
+Require Import Definitions.Axioms.
+
+Lemma TcHeapEmpty:
+  forall (heap : gmap HeapKey HeapVal) stty,
+    heap = ∅ ->
+    ST.Empty stty ->
+    TcHeap (heap, stty).
+Proof.
+  intros heap stty H1 H2.
+  unfold ST.Empty in *.
+   econstructor.
+  - intros.  unfold find_H in H.
+    assert(H3: ¬is_Some ((∅ : Heap) !! k)). apply lookup_empty_is_Some.
+    contradict H3. unfold is_Some. subst. exists v. assumption.
+  - intros. 
+    edestruct H2 with (a:=k) (e:=t).
+    unfold find_ST in H.       
+    apply STMapP.find_mapsto_iff.
+    assumption.
+  - intros.
+    edestruct H2 with (a:=k) (e:=t).
+    unfold find_ST in H.
+    apply STMapP.find_mapsto_iff.
+    assumption.
+Qed.
+
+  
+Lemma H_same_key_1: 
+  forall l v (heap : gmap HeapKey HeapVal),
+    (<[ l:=v ]> heap) !! l = Some v.
+Proof.
+  intros.
+  rewrite lookup_insert_Some.
+  left. split; reflexivity.
+Qed. 
+
+
+
+Lemma H_same_key_2:
+  forall l1 l2 v (heap : gmap HeapKey HeapVal),
+    l1 = l2 -> 
+    heap !! l1 = Some v ->
+    (<[ l2:=v ]> heap) !! l1 = Some v.
+Proof.
+  intros.
+  rewrite H.
+  rewrite  lookup_insert_Some.
+  left. split; reflexivity.
+Qed.
+
+
+Lemma H_diff_keys_1:
+  forall a b v v' (heap : gmap HeapKey HeapVal),   
+    a <> b ->
+    (<[ b:=v ]> heap) !! a = Some v' -> 
+    heap !! a = Some v'.
+Proof.
+  intros a b v v' e Hneq Hfind.
+  rewrite lookup_insert_Some in Hfind.
+  destruct Hfind as [[Ha Hb] | [Hc Hd]].
+  - contradict Hneq. auto.
+  - assumption.
+Qed.
+
+Lemma H_diff_keys_2:
+  forall a b v v' (heap : gmap HeapKey HeapVal),   
+    b <> a ->
+    heap !! a = Some v' ->
+    (<[ b:=v ]> heap) !! a = Some v'.
+Proof.
+  intros a b v v' e Hneq Hfind.
+  rewrite lookup_insert_Some.
+  right. split; [assumption | assumption].
+Qed.
+
+
+Lemma H_update_same_value: 
+  forall (heap : gmap HeapKey HeapVal) l v v',
+    (<[ l:=v ]> heap) !! l= Some v' -> v = v'.
+Proof.
+  intros heap l v v' Hfind. 
+  rewrite lookup_insert_Some in Hfind.
+  destruct Hfind as [[Ha Hb] | [Hc Hd]].
+  - assumption.
+  - contradict Hc. reflexivity.
+Qed.
+  
+
+Lemma H_same_domain:
+  forall stty heap, 
+    TcHeap (heap, stty) ->
+    (forall k v t,
+       find_ST k stty = None -> 
+       (forall (k0 : HeapKey) (v0 : Val),
+          find_H k0 (update_H (k, v) heap) = Some v0 ->
+          exists t0 : tau, find_ST k0 (update_ST (k, t) stty) = Some t0) /\
+       (forall (k0 : ST.key) (t0 : tau),
+          find_ST k0 (update_ST (k, t) stty) = Some t0 ->
+          exists v0 : Val, find_H k0 (update_H (k, v) heap) = Some v0)) /\
+    (forall k v t,
+       find_ST k stty = Some t ->
+       (forall (k0 : HeapKey) (v0 : Val),
+          find_H k0 (update_H (k, v) heap) = Some v0 ->
+          exists t0 : tau, find_ST k0 stty = Some t0) /\
+       (forall (k0 : ST.key) (t0 : tau),
+          find_ST k0 stty = Some t0 ->
+          exists v0 : Val, find_H k0 (update_H (k, v) heap) = Some v0)).
+Proof.
+  intros stty heap Hhp;
+  inversion_clear Hhp as [? ? TcHeap_STFind TcHeap_HFind TcHeap_tcVal]; split.
+  - intros k v t Hnone; split.
+    + intros k0 v0 Hfind'.
+      destruct k0 as [r0 l0]; destruct k as [r l];
+        destruct (eq_nat_dec l l0); destruct (eq_nat_dec r r0); subst;
+        try (apply H_diff_keys_1 in Hfind';
+             [ destruct (TcHeap_STFind (r0, l0) v0 Hfind') as [t0 STfind'];
+               exists t0; apply ST_diff_key_2;
+               [contradict n; inversion n; reflexivity | assumption] |
+               contradict n; inversion n; reflexivity ]).
+      * exists t. apply ST_same_key_1.
+    + intros k0 t0 STfind'; 
+      destruct k0 as [r0 l0];
+        destruct k as [r l];
+        destruct (eq_nat_dec l l0);
+        destruct (eq_nat_dec r r0); subst;
+        try ( apply ST_diff_keys_1 in STfind';
+            [ destruct (TcHeap_HFind (r0, l0) t0 STfind') as [v0 Hfind'];
+              exists v0;
+              apply H_diff_keys_2 | ]; simpl; intuition; apply n; now inversion H).
+      exists v. unfold find_H, update_H. apply H_same_key_1.
+  - intros k v t STfind; split.
+    + intros k0 v0 Hfind'.
+      destruct k0 as [r0 l0];
+        destruct k as [r l];
+        destruct (eq_nat_dec l l0);
+        destruct (eq_nat_dec r r0); subst;
+        try (apply H_diff_keys_1 in Hfind';
+           [destruct (TcHeap_STFind (r0, l0) v0 Hfind') as [t0 STfind']; now exists t0 |
+            simpl; intuition; apply n; now inversion H]).        
+      now exists t. 
+    + intros k0 t0 STfind'.
+      destruct k0 as [r0 l0];
+        destruct k as [r l];
+        destruct (eq_nat_dec l l0);
+        destruct (eq_nat_dec r r0); subst;
+        try (destruct (TcHeap_HFind (r0, l0) t0 STfind') as [v0 Hfind'];
+             exists v0; apply H_diff_keys_2;
+             simpl; intuition; apply n; now inversion H).                             
+      exists v; apply H_same_key_1.
+Qed.
+
+
+Lemma H_update_heap_fresh:
+  forall stty heap,
+    TcHeap (heap, stty) ->
+    (forall k v t,
+       find_ST k stty = None ->
+       TcVal (stty, v, t) ->
+       TcHeap (update_H (k, v) heap, update_ST (k, t) stty)).
+Proof. 
+  intros stty heap Hhp l v t Htc STfind.
+  inversion Hhp as [? ? TcHeap_STFind TcHeap_HFind TcHeap_tcVal]; subst; constructor.
+  - apply H_same_domain in Hhp. destruct Hhp as [Hnew ?]. edestruct Hnew; eauto.
+  - apply H_same_domain in Hhp. destruct Hhp as [Hnew ?]. edestruct Hnew; eauto.
+  - intros k v0 t0 Hfind' STfind'. destruct l as [r l]; destruct k as [r0 l0]. 
+    destruct (eq_nat_dec l l0);  destruct (eq_nat_dec r r0); subst;
+    try (eapply ST_diff_keys_1 in STfind'; eapply H_diff_keys_1 in Hfind'; eauto;
+         try (simpl; intuition; apply n; congruence); 
+         apply ext_stores__val with (stty:=stty);
+         [intros k1 t1 STfind''; destruct k1 as [r1 l1]; 
+           destruct (eq_nat_dec l0 l1);  destruct (eq_nat_dec r0 r1); subst;
+           try (apply ST_diff_key_2; [simpl; intuition; apply n; congruence | assumption]) |
+          now apply TcHeap_tcVal with (k := (r0, l0)) ] ).
+    apply ST_update_same_type in STfind'; 
+    apply H_update_same_value in Hfind'; simpl in *; subst.
+    apply ext_stores__val with (stty:=stty); auto.
+    intros k1 t1 STfind'. destruct k1 as [r1 l1].
+    destruct (eq_nat_dec l0 l1);  destruct (eq_nat_dec r0 r1); subst;
+    try (apply ST_diff_key_2; [ simpl; intuition; apply n; now inversion H | assumption] ).
+    rewrite STfind' in Htc. discriminate.
+Qed.
+
+
+
+Lemma H_update_heap_exists:
+  forall stty heap,
+    TcHeap (heap, stty) ->
+    (forall k v t,
+       find_ST k stty = Some t ->
+       TcVal (stty, v, t) ->
+       TcHeap (update_H (k, v) heap, stty)).
+Proof. 
+  intros stty heap Hhp l v t Htc STfind.
+  inversion Hhp as [? ? TcHeap_STFind TcHeap_HFind TcHeap_tcVal]; subst; constructor.
+  - apply H_same_domain in Hhp. destruct Hhp as [? Hupdate]. edestruct Hupdate; eauto.
+  - apply H_same_domain in Hhp. destruct Hhp as [? Hupdate]. edestruct Hupdate; eauto.
+  - intros k0 v0 t0 Hfind' STfind'. destruct l as [r l]; destruct k0 as [r0 l0]. 
+    destruct (eq_nat_dec l l0);  destruct (eq_nat_dec r r0); subst;
+    try (eapply H_diff_keys_1 in Hfind'; eauto; simpl; intuition; apply n; congruence).
+    apply H_update_same_value in Hfind'; subst.
+    rewrite STfind' in Htc. now inversion Htc. 
+Qed.
+
+
+Lemma EmptyTracePreservesHeap_1: 
+  forall h r env e same_h v' acts,
+    (h, r, env, e) ⇓ (same_h, v', acts) ->
+    acts = Phi_Nil ->
+    h ≡@{Heap} same_h.
+Proof.
+  intros h r env e same_h v' acts H Hnil.
+  dependent induction H; auto; inversion Hnil.
+  - eapply IHBigStep. reflexivity. auto. reflexivity.
+  - eapply IHBigStep; [reflexivity | auto | reflexivity]. 
+Qed.
+
+
+Lemma EMPTYTRACEPRESERVESHEAP_1 : 
+  forall h r env e same_h v' acts,
+    (h, r, env, e) ⇓ (same_h, v', acts) ->
+    acts = Phi_Nil ->
+    h ≡@{Heap} same_h.
+Proof.
+  intros h r env e same_h v' acts H Hnil.
+  dependent induction H; auto; inversion Hnil.
+  - eapply IHBigStep; [reflexivity | auto | reflexivity ].
+  - eapply IHBigStep; [reflexivity | auto | reflexivity ]. 
+Qed.
+
+
+Lemma Equal_heap_equal:
+  forall (heap1 heap2 : Heap),
+    heap1 = heap2 -> heap1 ≡@{Heap} heap2.
+Proof.
+  intros heap1 heap2 H. subst. auto.
+Qed.
+
+Lemma EqualHeaps:
+ forall heap_a heap_b store,
+   TcHeap (heap_a, store) ->
+   heap_a ≡@{Heap} heap_b ->
+   TcHeap (heap_b, store).
+Proof.
+  intros heap_a heap_b store HTcHeap HEqual.
+  unfold equiv, heap_equiv in HEqual; subst.
+  assumption.
+Qed.
+
+Lemma ReadOnlyTracePreservesHeap_1 : 
+  forall h env rho e same_h v' acts,
+    (h, env, rho, e) ⇓ (same_h, v', acts) ->
+    ReadOnlyPhi acts ->
+    h ≡@{Heap} same_h.
+Proof.
+intros h env rho e same_h v' acts H.
+  dependent induction H; intros;
+  try (solve [reflexivity]).
+  - inversion H2. inversion H5. subst.
+    assert (h=fheap) by (eapply  IHBigStep1; [reflexivity | auto | assumption]); subst.
+    assert (aheap=fheap)  by (symmetry; eapply IHBigStep2; auto); subst.
+   (eapply IHBigStep3; [reflexivity | reflexivity | assumption]).
+  - inversion H2; subst;
+    assert (h=fheap) by (eapply  IHBigStep1; [reflexivity | auto | assumption]); subst;
+    (eapply IHBigStep2; [reflexivity | reflexivity | assumption]). 
+  - inversion H5; subst. inversion H9; subst. 
+    assert (h = heap_mu1) by (eapply IHBigStep3; eauto).
+    assert (h = heap_mu2) by (eapply IHBigStep4; eauto). 
+    rewrite <- H6 in H2. rewrite <- H7 in H3.
+    assert (h = same_h) by (eapply ReadOnlyWalkSameHeap; eauto).
+    assumption.
+  - inversion H1; subst;
+    assert (h=cheap) by (eapply  IHBigStep1; [reflexivity | auto | assumption]).
+    eapply IHBigStep2; subst; [reflexivity | reflexivity | assumption].
+  - inversion H1; subst;
+    assert (h=cheap) by (eapply  IHBigStep1; [reflexivity | auto | assumption]).
+    eapply IHBigStep2; subst; [reflexivity | reflexivity | assumption].
+  - inversion H1; subst. inversion H5.
+  - inversion H2; subst; (eapply IHBigStep; [reflexivity | auto | assumption]).
+  - inversion H2; inversion H6.
+  - inversion H1; subst;
+    assert (h=lheap) by (eapply IHBigStep1; [reflexivity | auto |assumption]); subst;
+    (eapply IHBigStep2; [reflexivity | auto | assumption]).
+  - inversion H1; subst;
+    assert (h=lheap) by (eapply IHBigStep1; [reflexivity | auto |assumption]); subst;
+    (eapply IHBigStep2; [reflexivity | auto |assumption]).
+  - inversion H1; subst;
+    assert (h=lheap) by (eapply IHBigStep1; [reflexivity | auto |assumption]); subst;
+    (eapply IHBigStep2; [reflexivity | auto |assumption]).
+  - inversion H1; subst;
+    assert (h=lheap) by (eapply IHBigStep1; [reflexivity | auto |assumption]); subst;
+    (eapply IHBigStep2; [reflexivity | auto |assumption]).
+  - eapply EmptyTracePreservesHeap_1; eauto.
+  - eapply EmptyTracePreservesHeap_1. eauto. reflexivity.  
+Qed.   
+
+
+Lemma EmptyTracePreservesHeap_2 : 
+  forall h r env e same_h v acts,
+    (h, r, env, e) ⇓ (h, v, acts) ->
+    h ≡@{Heap} same_h ->
+    (same_h, r, env, e) ⇓ (same_h, v, acts).
+Proof.
+  intros h r env e same_h v' acts Dyn H.
+  unfold equiv, heap_equiv in H. now subst.
+Qed.
+
+Lemma EmptyTracePreservesHeap_3 : 
+  forall h r env e same_h v acts,
+    (same_h, r, env, e) ⇓ (same_h, v, acts) ->
+    (h, r, env, e) ⇓ (same_h, v, acts) ->
+    acts = Phi_Nil ->
+    (h, r, env, e) ⇓ (h, v, acts).
+Proof.
+  intros h r env e same_h v' acts Dyn Hheap Hnil.
+  apply EmptyTracePreservesHeap_1 in Hheap; unfold equiv, heap_equiv in Hheap;
+  now subst.
+Qed.
+
+Lemma EmptyTracePreservesHeap_4 : 
+  forall h r env e same_h v,
+    (h, r, env, e) ⇓ (same_h, v, Phi_Nil) ->
+    h ≡@{Heap} same_h.
+Proof.
+   intros h r env e same_h v' Dyn1.
+   dependent induction Dyn1; auto;  unfold equiv, heap_equiv.
+   eapply IHDyn1.
+   - reflexivity.
+   - econstructor.
+   - eapply IHDyn1.
+     + reflexivity.
+     + econstructor. 
+Qed.
+
+
+Lemma EmptyTracePreservesHeap_5 : 
+  forall h r env e  v,
+    (h, r, env, e) ⇓ (h, v, Phi_Nil) ->
+    exists same_h,  (same_h, r, env, e) ⇓ (h, v, Phi_Nil).
+Proof.
+  intros h r env e v H.
+  dependent induction H; exists h; econstructor; auto.
+  assumption. assumption.
+Qed.
+
+Lemma H_same_key_add_twice_1 :
+  forall r l r0 l0 v v0 (heap : gmap HeapKey HeapVal), 
+    (<[ (r0, l0):=v0 ]> (<[ (r, l):=v ]> heap)) !!  (r0, l0) =
+    (<[ (r0, l0):=v0 ]> heap) !! (r0, l0).
+Proof.
+  intros. rewrite H_same_key_1. rewrite H_same_key_1. reflexivity.
+Qed. 
+
+Lemma H_same_key_add_twice_2 :
+  forall k k0 v v0 (heap : gmap HeapKey HeapVal),
+    k <> k0 ->
+    ( <[ k:=v ]> (<[ k0:=v0 ]> heap)) !! k0 = ( <[k0:=v0]> heap) !! k0.
+Proof.
+  intros. rewrite H_same_key_1. apply H_diff_keys_2; [assumption | apply H_same_key_1]. 
+Qed.
+
+Lemma H_same_key_add_twice_3 :
+  forall k k0 v v0 (heap : gmap HeapKey HeapVal),
+    (<[k0:=v0]> (<[k:=v]> heap)) !! k0 = (<[k0:=v0]> heap) !! k0.
+Proof.
+  intros. rewrite H_same_key_1. symmetry. apply H_same_key_1. 
+Qed. 
+
+Lemma H_diff_key_add_twice_1 :
+  forall k0 k (heap : gmap HeapKey HeapVal) (v v0 e: Val), 
+    (<[k0:=v0]> heap) !! k0 = Some e ->
+    (<[k0:=v0]> (<[k:=v]> heap)) !! k0 = Some e.
+Proof.
+  intros k0 k heap v v0 e H.
+  rewrite H_same_key_add_twice_3. assumption.
+Qed.
+
+Lemma H_diff_key_add_twice_2 :
+  forall k0 k (heap : gmap HeapKey HeapVal) (v v0 e: Val),
+    k <> k0 ->
+    (<[ k:= v]> heap) !! k = Some e ->
+    (<[ k:=v]> (<[k0:=v0]> heap)) !! k = Some e.
+Proof.
+  intros k0 k heap v v0 e H. intro. 
+  rewrite H_same_key_add_twice_3. auto. 
+Qed.
+
+Lemma H_diff_key_add_comm_1:
+  forall k k1 k0 (heap : gmap HeapKey HeapVal) e v v0,
+    k1 <> k ->
+    k <> k0 ->
+    (<[ k0:=v0]> (<[k1:=v]> heap)) !! k = Some e ->
+    (<[k1:=v]> heap) !! k = Some e. 
+Proof.
+  intros  k k1 k0 heap e v v0 H1 H2 H3.
+  apply  H_diff_keys_1 in H3; assumption.
+Qed.
+
+Lemma H_diff_key_add_comm_2:
+  forall k k1 k0 (heap : gmap HeapKey HeapVal) e v v0,
+    k1 <> k ->
+    k <> k0 ->
+    (<[ k1:=v]>  heap) !! k = Some e ->
+    (<[ k1:=v]> (<[k0:=v0]> heap)) !! k = Some e. 
+Proof.
+  intros  k k1 k0 heap e v v0 H1 H2 H3.
+  apply  H_diff_keys_1 in H3.
+  - apply  H_diff_keys_2.
+   + assumption.
+   + apply  H_diff_keys_2.
+     * symmetry; assumption.
+     * assumption.
+  - symmetry; assumption.
+Qed.
+
+
+Lemma H_diff_keys_same_outer_k_2 :
+  forall r r0 r1 l l0 l1 v v0  (heap : gmap HeapKey HeapVal) e, 
+    (r0, l0) <> (r, l) -> 
+    ( <[(r, l):=v]> (<[(r0, l0):=v0]> heap)) !! (r1, l1) = Some e ->
+    (update_H (r0, l0, v0) (update_H (r, l, v) heap)) !! (r1, l1) = Some e.
+Proof.
+  intros  r r0 r1 l l0 l1 v v0 heap e H1 H2.
+  destruct (keys_eq_dec (r1, l1) (r0, l0)) as [K1 | K2];
+    destruct (keys_eq_dec (r1, l1) (r, l)) as [K3 | K4]; subst;
+    unfold keys_eq, Nat.eq in *; simpl in *.
+  - destruct K1 as [Ha Hb]; destruct K3 as [Hc Hd]; subst.
+    apply  H_diff_key_add_twice_2; auto.
+    apply  H_diff_keys_1 in H2; auto.   
+  - destruct K1 as [Ha Hb]. 
+    rewrite Ha in *.  rewrite Hb in *.
+    apply  H_diff_keys_1 in H2; auto. apply H_diff_key_add_twice_2; auto.
+  - destruct K3 as [Ha Hb]. 
+    rewrite Ha in *.  rewrite Hb in *.
+    apply  H_diff_keys_2; auto.
+    rewrite  H_same_key_add_twice_3 in H2; auto.
+  - apply  H_diff_keys_2; simpl.
+    + intuition.  apply H0; subst; inversion H; subst; reflexivity.
+    + apply  H_diff_keys_2; auto; simpl in *.
+      * intuition.  apply H3; subst; inversion H; subst; reflexivity.      
+      * apply  H_diff_keys_1 in H2. apply  H_diff_keys_1 in H2; auto.
+        { intuition.  apply H0; subst; inversion H; subst; reflexivity. }
+        { intuition. apply H3; subst; inversion H; subst; reflexivity.  }
+Qed.
+
+
+Lemma H_monotonic_updates:
+  forall phi phi' (heap heap' : gmap HeapKey HeapVal),
+     (phi, heap) ===> (phi', heap') ->
+     forall r l,
+       find_H (r, l) heap ≠ None ->
+       find_H (r, l) heap' ≠ None.
+Proof.
+  intros phi phi' heap heap' H.  
+  dependent induction H; intros; unfold find_H, update_H in *; simpl in *.
+  - intro. apply H.
+    apply lookup_insert_None in H0. destruct H0.
+    assumption.
+  - intro. apply H0. assumption.
+  - intro. apply H0.
+    apply lookup_insert_None in H1. destruct H1.
+    assumption.
+  - apply IHPhi_Heap_Step with (phi:=phi1) (heap:=heap) (phi':=phi1').
+    + reflexivity.
+    + reflexivity.
+    + assumption.
+  - apply IHPhi_Heap_Step with (phi:=phi2) (heap:=heap) (phi':=phi2'). 
+    + reflexivity.
+    + reflexivity.
+    + assumption.
+  - assumption.
+  - apply IHPhi_Heap_Step with (phi:=phi1) (heap:=heap) (phi':=phi1').
+    + reflexivity.
+    + reflexivity.
+    + assumption.
+  - apply IHPhi_Heap_Step with (phi:=phi2) (heap:=heap) (phi':=phi2'). 
+    + reflexivity.
+    + reflexivity.
+    + assumption.
+ - assumption.
+Qed.
