Proofs/TypeFacts.v
@@ -1,0 +1,1018 @@
+Require Import Coq.Program.Equality.
+Require Import Coq.Sets.Ensembles.
+Require Import Definitions.StaticActions.
+Require Import Definitions.ComputedActions.
+Require Import Definitions.Regions.
+Require Import Definitions.Types.
+Require Import Definitions.Keys.
+Require Import Definitions.Values.
+Require Import Definitions.Axioms.
+Require Import Proofs.RegionFacts.
+Require Import Proofs.EffectFacts.
+Require Import Proofs.LocallyNameless.
+
+Module STMapP := FMapFacts.Facts ST.
+Module STRaw := ST.Raw.
+Module STProofs := ST.Raw.Proofs.
+
+Definition find_type_ext_stores_def  := 
+   forall stty stty' l (t' : tau),
+      ST.find l stty = Some t' ->
+      ST.find l stty' = Some t' -> 
+      ST.find l stty =  ST.find l stty'.
+
+Lemma find_type_ext_stores: find_type_ext_stores_def.  
+Proof.
+  intros stty stty' l t' H1 H2.
+  rewrite <- H1 in H2.
+  symmetry in H2.
+  assumption.
+Qed.
+
+
+Lemma ST_same_key_1:
+  forall t l ty stty, 
+    ST.find (elt := t) l (ST.add l ty stty) = Some ty.
+Proof.
+  intros; rewrite <- STMapP.find_mapsto_iff. now apply ST.add_1.
+Qed. 
+
+Lemma ST_diff_keys_1:
+  forall t a b v v' e,   
+    a <> b ->
+    ST.find (elt := t) a (ST.add b v e) = Some v' -> 
+    ST.find (elt := t) a e = Some v'.
+Proof.
+  intros  t a b v v' e H1 H2. 
+  rewrite <- STMapP.find_mapsto_iff in H2. rewrite -> STMapP.add_mapsto_iff in H2.
+  intuition.
+  - destruct a, b; simpl in *; subst; intuition.
+  - now rewrite -> STMapP.find_mapsto_iff in H2.
+Qed.
+
+
+Lemma ST_diff_key_2:
+  forall t a b v v' e,   
+    b <> a ->
+    ST.find (elt := t) a e = Some v' ->
+    ST.find (elt := t) a (ST.add b v e) = Some v'.
+Proof.
+  intros. 
+  rewrite <- STMapP.find_mapsto_iff. rewrite -> STMapP.add_mapsto_iff.
+  destruct a, b; simpl.
+  right. intuition. now rewrite STMapP.find_mapsto_iff.
+Qed.
+
+
+Lemma ST_update_same_type:
+  forall stty l0 t t0,
+  ST.find (elt:=tau) l0 (ST.add l0 t stty) = Some t0 -> 
+  t = t0.
+Proof.
+  intros stty l0 t t0 H. 
+  rewrite ST_same_key_1 in H. inversion H. reflexivity.
+Qed.
+
+
+
+Definition get_store_typing_val {A B:Type} (p : Sigma * A * B) : Sigma   
+  := fst (fst p).
+
+Definition get_store_typing_env {A B C:Type} (p : Sigma * A * B * C) : Sigma   
+  := fst (fst (fst p)).
+
+Definition mk_TcVal_ext_store_ty (p : Sigma * Val * tau) (stty' : Sigma)
+  := TcVal (stty', snd (fst p), snd p).
+
+Definition mk_TcEnv_ext_store_ty (p : Sigma * Rho * Env * Gamma) (stty' : Sigma)
+  := TcEnv (stty', snd (fst (fst p)), snd (fst p), snd p).
+
+Lemma ext_stores__exp__bt__aux:
+  (forall p, TcExp p ->
+             match p with (ctxt, rgns, e, t, eff) => 
+                TcExp (ctxt, rgns, e, t, eff)
+             end)
+    /\
+  (forall p, BackTriangle p ->
+             match p with (ctxt, rgns, rho, ec, ee) => 
+                BackTriangle (ctxt, rgns, rho, ec, ee)
+             end)
+   /\  
+  (forall p,
+        TcVal p ->        
+        forall stty stty',
+        (forall l t', find_ST l stty = Some t' -> find_ST l stty' = Some t') -> 
+        get_store_typing_val p = stty -> mk_TcVal_ext_store_ty p stty') 
+  /\
+     (forall p,
+        TcEnv p ->           
+        forall stty stty',
+        (forall l t', find_ST l stty = Some t' -> find_ST l stty' = Some t') -> 
+        get_store_typing_env p = stty -> mk_TcEnv_ext_store_ty p stty').
+Proof.
+  apply tc__xind; try (solve [econstructor;eauto] ).
+  - intros. 
+    unfold mk_TcVal_ext_store_ty, 
+           mk_TcEnv_ext_store_ty, 
+           get_store_typing_val, 
+           get_store_typing_env in *; simpl in *.
+    subst.
+    econstructor; eauto.
+  - intros.
+     unfold mk_TcVal_ext_store_ty, 
+           mk_TcEnv_ext_store_ty, 
+           get_store_typing_val, 
+           get_store_typing_env in *; simpl in *.
+    subst.
+    econstructor; eauto.
+  - intros.
+    unfold mk_TcVal_ext_store_ty, 
+           mk_TcEnv_ext_store_ty, 
+           get_store_typing_val, 
+           get_store_typing_env in *; simpl in *.
+    subst.
+    econstructor; eauto.
+  - intros.
+    unfold mk_TcVal_ext_store_ty, 
+           mk_TcEnv_ext_store_ty, 
+           get_store_typing_val, 
+           get_store_typing_env in *; simpl in *.
+    subst.
+    econstructor; eauto.
+Qed.
+
+Lemma ext_stores__val:
+   forall stty stty',
+     (forall l t', find_ST l stty = Some t' -> find_ST l stty' = Some t') -> 
+     (forall v t, TcVal (stty, v, t) -> 
+      TcVal (stty', v, t)).
+Proof.
+  intros.
+  eapply (match ext_stores__exp__bt__aux with conj _ (conj _ (conj F _)) =>
+   F (stty, v, t) end); eauto.
+Qed.
+
+Lemma ext_stores__env:
+   forall stty stty',
+     (forall l t', find_ST l stty = Some t' -> find_ST l stty' = Some t') -> 
+     (forall rho env ctxt, TcEnv (stty, rho, env, ctxt) ->  
+      TcEnv (stty', rho, env, ctxt)).
+Proof.
+  intros.
+  eapply (match ext_stores__exp__bt__aux 
+          with conj _ (conj _ (conj _ F)) =>
+               F (stty, rho, env, ctxt) end); eauto.
+Qed.
+
+
+Lemma update_rho: forall rho rgns x v,
+                    TcRho (rho, rgns) ->
+                    not_set_elem rgns x ->
+                    TcRho (update_R (x, v) rho, set_union rgns (singleton_set x)).
+Proof.
+  intros rho rgns x v HRho HFresh.
+  unfold update_R; simpl. 
+  econstructor.  
+  intro r. split.
+  - inversion_clear HRho as [rho' rgns' HRgn'  HRho''].
+    destruct (AsciiVars.eq_dec x r) as [c | c].
+    + unfold AsciiVars.eq in c; intros; subst.
+      unfold set_elem, set_union, singleton_set.
+      apply Ensembles.Union_intror.
+      apply Ensembles.In_singleton.
+    + destruct (HRgn' r).
+      intro. 
+      apply H0 in H. 
+      * eapply R_diff_key_3 in H1; auto.  
+        apply Ensembles.Union_introl. 
+        apply HRgn'. assumption.
+      * eapply R_diff_key_3 in H1; auto.  
+  - inversion_clear HRho as [rho' rgns' HRgn'  HRho''].
+    destruct (AsciiVars.eq_dec x r) as [c | c].
+    + unfold AsciiVars.eq in c; intros; subst.
+      apply RMapP.in_find_iff. apply RMapP.add_in_iff. intuition.
+    + destruct (HRgn' r).
+      intro. apply H0 in H. 
+      * rewrite <- RMapP.in_find_iff.  rewrite RMapP.add_in_iff.
+        right. rewrite RMapP.in_find_iff. 
+        assumption.
+      * destruct H1; [apply H0; assumption | inversion H1; subst; contradict c; reflexivity].
+Qed.
+
+
+Definition subst_in_type := fun x r ty => subst_type x (Rgn2_Const true false r) ty.
+
+
+
+Lemma subst_type_rgn_comm_2:
+  forall r k1 k2 v1 v2,
+    k1 <> k2 ->
+    subst_rgn k1 (Rgn2_Const true false v1) (subst_rgn k2 (Rgn2_Const true false v2) r) =
+    subst_rgn k2 (Rgn2_Const true false v2) (subst_rgn k1 (Rgn2_Const true false v1) r).
+Proof.
+  intros r k1 k2 v1 v2 H.
+  unfold Region_in_Type in r.
+  dependent induction r; try (solve [simpl; reflexivity ]).
+  unfold subst_rgn. destruct (AsciiVars.eq_dec k1 k2).
+  - inversion e. contradiction.
+  - simpl. destruct (AsciiVars.eq_dec k2 v).
+    + assert (~ AsciiVars.eq k1 v) by (inversion e; congruence).
+      unfold  AsciiVars.eq in *.
+      destruct (AsciiVars.eq_dec k1 v).
+      * now absurd (k1=v).
+      * inversion e; subst; now destruct (AsciiVars.eq_dec v v).
+    + destruct (AsciiVars.eq_dec k1 v); [reflexivity |].
+      now destruct (AsciiVars.eq_dec k2 v).
+Qed.  
+
+
+Lemma subst_type_sa_comm_2:
+  forall sa k1 k2 v1 v2,
+    k1 <> k2 ->
+    subst_sa k1 (Rgn2_Const true false v1) (subst_sa k2 (Rgn2_Const true false v2) sa) =
+    subst_sa k2 (Rgn2_Const true false v2) (subst_sa k1 (Rgn2_Const true false v1) sa).
+Proof.
+  intros sa k1 k2 v1 v2 H.
+  destruct sa; simpl; apply f_equal; apply subst_type_rgn_comm_2; auto.
+Qed.
+
+Lemma subst_type_eps_comm_2 : forall (k1 : R.key) (v1 : RgnId) (k2 : R.key) (v2 : RgnId) (e : Epsilon),
+                                k1 <> k2 ->
+                                subst_eps k1 (Rgn2_Const true false v1) (subst_eps k2 (Rgn2_Const true false v2) e) =
+                                subst_eps k2 (Rgn2_Const true false v2) (subst_eps k1 (Rgn2_Const true false v1) e).
+Proof.
+  intros k1 v1 k2 v2 e H. unfold subst_eps.
+  apply Extensionality_Ensembles; unfold Same_set, Included.
+  split; intros; unfold Ensembles.In in *; destruct H0 as [x' [[x'' [H1 H2]] H3]];
+  subst; repeat (eexists || split || subst); eauto using subst_type_sa_comm_2.
+Qed.
+
+
+Lemma subst_type_type_comm_2 : forall (k1 : R.key) (v1 : RgnId) (k2 : R.key) (v2 : RgnId) (b : tau),
+                          k1 <> k2 -> 
+                          subst_in_type k1 v1 (subst_in_type k2 v2 b) = subst_in_type k2 v2 (subst_in_type k1 v1 b).
+Proof.
+  intros k1 v1 k2 v2 b H.
+  unfold subst_in_type.
+  induction b; simpl; try (solve [simpl; reflexivity ]).
+  - f_equal; [apply IHb1 | apply IHb2].
+  - f_equal; [ | apply IHb].
+    now apply  subst_type_rgn_comm_2.
+  - f_equal; [ apply IHb1 | |  apply IHb2 | |  apply IHb3];
+      eauto using subst_type_eps_comm_2.
+  - f_equal; [ | apply IHb]; eauto using subst_type_eps_comm_2.
+Qed.
+
+
+Lemma subst_add_comm_rgn :
+  forall k v rho ,
+    ~ R.In (elt:=RgnId) k rho ->
+    forall rgn, 
+      fold_subst_rgn (R.add k v rho) rgn = fold_subst_rgn rho (subst_in_rgn k v rgn).
+Proof.
+  intros k v rho H rgn.
+   apply fold_add_type. 
+   - assumption.
+   - intros k0 v0 b0 H'.
+     rewrite subst_type_rgn_comm_2.
+     + reflexivity.
+     + intro; subst.
+       destruct H.
+       apply RMapProp.F.elements_in_iff.
+       exists v0.
+       apply RMapProp.F.elements_mapsto_iff.
+       assumption.
+Qed.
+
+Lemma subst_add_comm_sa :
+  forall k v rho ,
+    ~ R.In (elt:=RgnId) k rho ->
+    forall sa, 
+      fold_subst_sa (R.add k v rho) sa = fold_subst_sa rho (subst_in_sa k v sa).
+Proof.
+  intros k v rho H sa.
+  unfold fold_subst_sa.
+  induction sa; simpl; f_equal; apply subst_add_comm_rgn; assumption.
+Qed.
+
+
+Lemma subst_add_comm_eff :
+  forall k v rho ,
+    ~ R.In (elt:=RgnId) k rho ->
+    forall eff, 
+      fold_subst_eps (R.add k v rho) eff = fold_subst_eps rho (subst_in_eff k v eff). 
+Proof.
+  intros k v rho H eff. unfold fold_subst_eps.
+  apply Extensionality_Ensembles; unfold Same_set, Included. 
+  intuition; unfold Ensembles.In in *. 
+  - destruct H0 as [sa [H1 H2]].
+    exists (subst_in_sa k v sa).
+    rewrite <- subst_add_comm_sa; eauto.
+    intuition.
+    unfold subst_in_eff, subst_in_sa.
+    unfold subst_eps, subst_sa.
+    exists sa. intuition.
+  - destruct H0 as [sa [H1 H2]].
+    unfold subst_in_eff, subst_eps in H1.
+    destruct H1 as [sa' [H3 H4]]. subst.
+    exists sa'. rewrite subst_add_comm_sa; eauto.
+Qed.
+
+
+Lemma subst_add_comm :
+  forall k v rho ,
+    ~ R.In (elt:=RgnId) k rho ->
+    forall ty, 
+      subst_rho (R.add k v rho) ty = subst_rho rho (subst_in_type k v ty). 
+Proof.
+  intros k v rho H ty.
+  (*unfold subst_rho, subst_in_type.*)
+  apply fold_add_type.  
+  - assumption.
+  - intros k0 v0 b0 H'.
+    rewrite subst_type_type_comm_2.
+    + reflexivity.
+    + intro; subst.
+      destruct H.
+      apply RMapProp.F.elements_in_iff.
+      exists v0.
+      apply RMapProp.F.elements_mapsto_iff.
+      assumption.
+Qed.
+
+Lemma not_set_elem_not_in_rho: forall rho rgns x,
+                                 TcRho (rho, rgns) ->
+                                 not_set_elem rgns x ->
+                                 ~ R.In (elt:=RgnId) x rho.
+Proof.
+  intros rho rgns  x HRho H .
+  inversion_clear HRho as [rho' rgns' HRgn' HVal''].
+  unfold not_set_elem in H. unfold Ensembles.Complement in H.
+  intro. 
+  apply RMapP.in_find_iff in H0.
+  eapply HRgn' in H0. contradiction.
+Qed.
+
+
+
+Lemma NotFreeInEmptyEps:
+  forall x,
+    ~ free_rgn_vars_in_eps (Empty_set StaticAction) x.
+Proof.
+  intro x. intro. 
+  unfold free_rgn_vars_in_eps, empty_set in H.
+  destruct H as [sa]. destruct H.
+  inversion H.
+Qed.
+
+
+Module EProofs := Raw.Proofs.
+Module EMapP := FMapFacts.Facts E.
+
+
+Lemma E_same_key:
+  forall t x v e, 
+    E.find (elt := t) x (E.add x v e) = Some v.
+Proof.
+  intros. rewrite <- EMapP.find_mapsto_iff. rewrite -> EMapP.add_mapsto_iff.
+  left. intuition. 
+Qed.  
+
+Lemma E_diff_key_1:
+  forall t a b v v' e,   
+    a <> b ->
+    E.find (elt := t) a (E.add b v e) = Some v' -> 
+    E.find (elt := t) a e = Some v'.
+Proof.
+  intros. 
+  rewrite <- EMapP.find_mapsto_iff in H0. rewrite -> EMapP.add_mapsto_iff in H0.
+  destruct H0; destruct H0; [destruct H | rewrite -> EMapP.find_mapsto_iff in H1]; auto.
+Qed.
+
+
+Lemma E_diff_key_2:
+  forall t a b v v' e,   
+    b <> a ->
+    E.find (elt := t) a e = Some v' ->
+    E.find (elt := t) a (E.add b v e) = Some v'.
+Proof.
+  intros. 
+  rewrite <- EMapP.find_mapsto_iff. rewrite -> EMapP.add_mapsto_iff.
+  right; split; [exact H | now rewrite EMapP.find_mapsto_iff ].
+Qed.
+
+
+Lemma ExtendedTcInv_2:
+  forall ctxt rgns f x tyx effe tyc effc, 
+    TcInc (ctxt, rgns)->
+    included (frv tyx) rgns ->
+    included (frv (Ty2_Arrow tyx effc tyc effe Ty2_Effect)) rgns ->
+    TcInc (update_rec_T (f, Ty2_Arrow tyx effc tyc effe Ty2_Effect) (x, tyx) ctxt, rgns).
+Proof.
+  intros ctxt rgns f x tyx effe tyc effc HInc HFind1 HFind2.
+  inversion HInc as [? ? HFrv]; subst.
+  unfold included, Included in *.
+  econstructor.    
+  intros. unfold find_T in H, HFrv.
+  unfold update_rec_T in H. simpl in H.
+  destruct (AsciiVars.eq_dec x0 x) as [c | c].
+  - inversion c; subst.
+    rewrite E_same_key in H.
+    inversion H; subst.
+    do 2 intro. eapply HFind1. assumption.
+  - destruct (AsciiVars.eq_dec x0 f) as [d | d].
+    + inversion d; subst.
+      unfold AsciiVars.eq in c.
+      eapply E_diff_key_1 in H; auto.
+      rewrite E_same_key in H.
+      inversion H; subst.
+      do 2 intro. eapply HFind2. assumption.
+    + eapply E_diff_key_1 in H; eauto. 
+      eapply E_diff_key_1 in H; eauto.
+      do 2 intro.
+      eapply HFrv; eauto.
+Qed.
+
+
+Lemma subst_rho_free_vars_eps:
+  forall rho x (e : Ensemble StaticAction),
+   R.find (elt:=RgnId) x rho = None ->  
+   not_set_elem (free_rgn_vars_in_eps (fold_subst_eps rho e)) x ->
+   not_set_elem (free_rgn_vars_in_eps e) x.
+Proof.
+  intro rho. destruct rho. induction this; intros x e' H1 H2.
+  - intro. apply H2. unfold In in *. clear H2.
+    unfold free_rgn_vars_in_eps in *.
+    destruct H as [sa [Ha Hb]]. 
+    exists sa; intuition.
+    unfold fold_subst_eps. 
+    exists sa. intuition. 
+    unfold fold_subst_sa, fold_subst_rgn, subst_rgn, R.fold, R.Raw.fold ; simpl.
+    induction sa; reflexivity.
+  - inversion is_bst; subst. 
+    destruct (AsciiVars.compare x k); subst.
+    + eapply IHthis1 with (is_bst:=H5); eauto.
+      * eapply find_rho_1; eauto.
+      * intro. apply H2. unfold In in *.
+        eapply subst_rho_free_vars_eps_aux_1; eauto.
+    + inversion e0; subst.
+      intro. apply H2. unfold In in *. 
+      unfold free_rgn_vars_in_eps, fold_subst_eps in *.
+      destruct H as [sa [Ha Hb]].
+      exists sa. split; [| assumption].
+      exists sa. split; [assumption|]. 
+      apply equal_fold_subst_sa; auto.
+    + eapply IHthis2  with (is_bst:=H7); eauto. 
+      * eapply find_rho_2; eauto.  
+      * intro. apply H2. unfold In in *.
+        eapply subst_rho_free_vars_eps_aux_2. assumption.
+        eassumption.
+Qed.
+
+Lemma subst_rho_free_vars :
+  forall t rho x,
+    x # subst_rho rho t ->
+    R.find (elt:=nat) x rho = None ->
+    x # t.
+Proof.
+  intro t. dependent induction t; intros rho x H1 H2. 
+  - rewrite subst_rho_natural in H1. assumption.
+  - rewrite subst_rho_boolean in H1. assumption.
+  - rewrite subst_rho_effect in H1. assumption.
+  - rewrite subst_rho_unit in H1. assumption.
+  - rewrite subst_rho_pair in H1. simpl in *.
+    apply subst_rho_free_vars_union_1 in H1; auto. destruct H1.
+    apply subst_rho_free_vars_union_2.
+    split; [eapply IHt1 | eapply IHt2]; eauto.
+  - rewrite subst_rho_tyref in H1. simpl in *.
+    apply subst_rho_free_vars_union_1 in H1; auto. destruct H1.
+    apply subst_rho_free_vars_union_2.
+    split; [ eapply subst_rho_free_vars_rgn | eapply IHt]; eauto.
+  - rewrite subst_rho_arrow in H1. simpl in *.
+    eapply subst_rho_free_vars_union_1 in H1. destruct H1.
+    eapply subst_rho_free_vars_union_1 in H0. destruct H0.
+    eapply subst_rho_free_vars_union_1 in H0. destruct H0.
+    eapply subst_rho_free_vars_union_1 in H1. destruct H1.
+    apply subst_rho_free_vars_union_2.
+    split;  [eapply IHt1 | apply subst_rho_free_vars_union_2]; eauto.
+    split.
+    + apply subst_rho_free_vars_union_2.
+      split; [ eapply subst_rho_free_vars_eps | eapply subst_rho_free_vars_eps]; eauto. 
+    + eapply subst_rho_free_vars_union_2.
+      split; [eapply IHt2 | eapply IHt3]; eauto. 
+  - rewrite subst_rho_forallrgn in H1; simpl in *.
+    eapply subst_rho_free_vars_union_1 in H1. destruct H1.
+    eapply subst_rho_free_vars_union_2.
+    split; [ eapply subst_rho_free_vars_eps | eapply IHt]; eauto.
+Qed.
+
+
+Lemma TypedExpressionFrv :
+  forall ctxt rgns e t eff,
+  TcInc (ctxt, rgns) ->
+  TcExp (ctxt, rgns, e, t, eff) ->
+  included (frv t) rgns /\ included (free_rgn_vars_in_eps eff) rgns.
+Proof. 
+  intros ctxt rgns e t eff HInc HExp.  
+  generalize dependent HInc.  
+  dependent induction HExp;
+  intros HInc; unfold included, Included, In;
+  try (solve [intuition; [inversion H | contradict H; apply NotFreeInEmptyEps] ]). 
+  - inversion HInc as [? ? HFrv]; subst.
+    intuition; eapply HFrv; eauto. contradict H0; apply NotFreeInEmptyEps.
+  - inversion HInc as [? ? HFrv]; subst.
+    assert (H' : included (frv tyc) rgns /\ included (free_rgn_vars_in_eps effc) rgns).
+    { eapply IHHExp1; eauto. 
+      simpl in H0. 
+      assert (H': included (frv tyx) rgns) 
+        by  (apply IncludedUnion_Name_1 in H0; destruct H0; assumption). 
+      apply ExtendedTcInv_2; eauto. }
+     
+    { assert (H'' : included (frv Ty2_Effect) rgns /\ 
+                    included (free_rgn_vars_in_eps effe) rgns).
+      eapply IHHExp2; eauto.
+      - simpl in H0. 
+        assert (H''': included (frv tyx) rgns) 
+          by  (apply IncludedUnion_Name_1 in H0; destruct H0; assumption).  
+        apply ExtendedTcInv_2; eauto. 
+      - split; auto.
+        intro. intro. contradict H1. apply NotFreeInEmptyEps. }
+  - inversion HInc as [? ? HFrv]; subst.
+    assert (H' : included (frv tyr) (set_union rgns (singleton_set x)) /\ 
+                 included (free_rgn_vars_in_eps effr) (set_union rgns (singleton_set x))).
+    { eapply IHHExp; eauto.
+      econstructor.
+      intros. intro. intros.
+      apply Union_introl. eapply HFrv; eauto. } 
+    split; simpl.
+    intuition.
+    + unfold included, Included in *.
+      destruct H5; unfold In in *.
+      * eapply RegionAbsFrv_1; eauto.
+      * eapply RegionAbsFrv_3; eauto.
+    + intros. contradict H3. apply NotFreeInEmptyEps.
+  - assert (H' : included (frv (Ty2_Arrow tya effc t effe Ty2_Effect)) rgns /\ 
+                 included (free_rgn_vars_in_eps efff) rgns) by (eapply IHHExp1; eauto).
+    assert (H'' : included (frv tya) rgns /\ 
+                  included (free_rgn_vars_in_eps effa) rgns) by (eapply IHHExp2; eauto).
+    destruct H' as [H2 H3].
+    destruct H'' as [H4 H5].
+    split.
+    + do 2 intro. apply H2. simpl.
+      apply Union_intror. apply Union_intror. apply Union_introl. assumption.
+    + intro. apply IncludedUnion_Static_Action_4; [apply IncludedUnion_Static_Action_4 |].
+      * apply H3.
+      * apply H5.
+      * intro. apply H0. auto.
+  - inversion HInc as [? ? HFrv]; subst.
+    assert (H' : included (frv (Ty2_ForallRgn effr tyr)) rgns /\ 
+                 included (free_rgn_vars_in_eps efff) rgns).
+    eapply IHHExp; eauto.
+    destruct H' as [H2 H3].
+    split.
+    + simpl in H2.
+      apply IncludedUnion_Name_1 in H2. 
+      destruct H2 as [H4 H5].
+      apply RegionAppFrv_1; auto.
+    + intro. apply IncludedUnion_Static_Action_4.
+      * apply H3.
+      * apply H1.
+  -inversion HInc as [? ? HFrv]; subst.
+    assert (H' : included (frv ( Ty2_Arrow tya effc tyc effe Ty2_Effect)) rgns /\ 
+                 included (free_rgn_vars_in_eps efff) rgns).
+    eapply IHHExp1; eauto.
+    assert (H'' : included (frv tya) rgns /\ 
+                  included (free_rgn_vars_in_eps effa) rgns).
+    eapply IHHExp2; eauto.
+    destruct H' as [H1 H2].
+    destruct H'' as [H3 H4].
+    split.
+    + do 2 intro. inversion H0.
+    + intro. apply IncludedUnion_Static_Action_4; [apply IncludedUnion_Static_Action_4 |].
+      * apply H2.
+      * apply H4. 
+      * apply H. 
+  - assert (H1 : included (frv ty1) rgns /\ included (free_rgn_vars_in_eps eff1) rgns)
+      by (eapply IHHExp1; eauto).
+    assert (H2 : included (frv ty2) rgns /\ included (free_rgn_vars_in_eps eff2) rgns)
+      by (eapply IHHExp2; eauto).
+    assert (H3 : included (frv ty3) rgns /\ included (free_rgn_vars_in_eps eff3) rgns)
+      by (eapply IHHExp3; eauto).
+    assert (H4 : included (frv ty4) rgns /\ included (free_rgn_vars_in_eps eff4) rgns)
+      by (eapply IHHExp4; eauto).
+    split.
+    + do 2 intro. simpl in H.
+      destruct H.
+      * destruct H1. apply H0. assumption.
+      * destruct H2. apply H0. assumption.
+    + intro. apply IncludedUnion_Static_Action_4; 
+             [apply IncludedUnion_Static_Action_4; [apply IncludedUnion_Static_Action_4 |] |];
+             [destruct H3 | destruct H4 | destruct H2 | destruct H1]; apply H0. 
+  - assert (H1 : included (frv t0) rgns /\ included (free_rgn_vars_in_eps veff) rgns)
+      by (eapply IHHExp; eauto).
+    destruct H1 as [H2 H3].
+    split.
+    + do 2 intro. simpl in H.
+      rewrite EmptyUnionisEmptySet_Name_Left in H.
+      apply H2. assumption.
+    + intro. apply IncludedUnion_Static_Action_4; [apply H3 |].
+      simpl. apply H0. 
+  - assert (H2 : included (frv (Ty2_Ref (mk_rgn_type (Rgn2_Const true false s)) t)) rgns /\ 
+                 included (free_rgn_vars_in_eps aeff) rgns)
+      by (eapply IHHExp; eauto).
+    destruct H2 as [H3 H4].
+    split.
+    + do 2 intro. apply H3; simpl.
+      apply Union_intror. assumption.
+    + intro. apply IncludedUnion_Static_Action_4; [apply H4 |].
+      simpl. apply H1.
+  - assert (H2 : included (frv (Ty2_Ref (mk_rgn_type (Rgn2_Const true false s)) t0)) rgns
+                 /\ included (free_rgn_vars_in_eps aeff) rgns)
+      by (eapply IHHExp1; eauto).
+    assert (H3 : included (frv t0) rgns /\ 
+                 included (free_rgn_vars_in_eps veff) rgns)
+      by (eapply IHHExp2; eauto).
+     destruct H2 as [H4 H5].
+     destruct H3 as [H6 H7].
+     split.
+     + do 2 intro. inversion H.
+     + intro.  apply IncludedUnion_Static_Action_4; [ apply IncludedUnion_Static_Action_4  |].
+       * apply H5.
+       * apply H7. 
+       * simpl. apply H1. 
+  - assert (H1 : included (frv Ty2_Boolean) rgns /\ 
+                 included (free_rgn_vars_in_eps eff0) rgns)
+      by (eapply IHHExp1; eauto).
+    assert (H2 : included (frv t) rgns /\ 
+                 included (free_rgn_vars_in_eps eff1) rgns)
+      by (eapply IHHExp2; eauto).
+    assert (H3 : included (frv t) rgns /\ 
+                 included (free_rgn_vars_in_eps eff2) rgns)
+      by (eapply IHHExp3; eauto).
+    destruct H1 as [H4 H5].
+    destruct H2 as [H6 H7].
+    destruct H3 as [H8 H9].
+    split.
+    + do 2 intro. apply H6. assumption.
+    + intro.  apply IncludedUnion_Static_Action_4; [ | apply IncludedUnion_Static_Action_4 ].
+      * apply H5.
+      * apply H7.
+      * apply H9. 
+  - assert (H1 : included (frv Ty2_Natural) rgns /\ 
+                 included (free_rgn_vars_in_eps eff1) rgns)
+      by (eapply IHHExp1; eauto).
+    assert (H2 : included (frv Ty2_Natural) rgns /\ 
+                 included (free_rgn_vars_in_eps eff2) rgns)
+      by (eapply IHHExp2; eauto).
+    destruct H1 as [H3 H4].
+    destruct H2 as [H5 H6].
+    split.
+    + do 2 intro. apply H3. assumption.
+    + intro. apply IncludedUnion_Static_Action_4; [apply H4 | apply H6].
+  - assert (H1 : included (frv Ty2_Natural) rgns /\ 
+                 included (free_rgn_vars_in_eps eff1) rgns)
+      by (eapply IHHExp1; eauto).
+    assert (H2 : included (frv Ty2_Natural) rgns /\ 
+                 included (free_rgn_vars_in_eps eff2) rgns)
+      by (eapply IHHExp2; eauto).
+    destruct H1 as [H3 H4].
+    destruct H2 as [H5 H6].
+    split.
+    + do 2 intro. apply H3. assumption.
+    + intro. apply IncludedUnion_Static_Action_4; [apply H4 | apply H6].
+  - assert (H1 : included (frv Ty2_Natural) rgns /\ 
+                 included (free_rgn_vars_in_eps eff1) rgns)
+      by (eapply IHHExp1; eauto).
+    assert (H2 : included (frv Ty2_Natural) rgns /\ 
+                 included (free_rgn_vars_in_eps eff2) rgns)
+      by (eapply IHHExp2; eauto).
+    destruct H1 as [H3 H4].
+    destruct H2 as [H5 H6].
+    split.
+    + do 2 intro. apply H3. assumption.
+    + intro. apply IncludedUnion_Static_Action_4; [apply H4 | apply H6].
+  - assert (H1 : included (frv Ty2_Natural) rgns /\ 
+                 included (free_rgn_vars_in_eps eff1) rgns)
+      by (eapply IHHExp1; eauto).
+    assert (H2 : included (frv Ty2_Natural) rgns /\ 
+                 included (free_rgn_vars_in_eps eff2) rgns)
+      by (eapply IHHExp2; eauto).
+    destruct H1 as [H3 H4].
+    destruct H2 as [H5 H6].
+    split.
+    + do 2 intro. apply H3. assumption.
+    + intro. apply IncludedUnion_Static_Action_4; [apply H4 | apply H6].
+  - assert (H1 : included (frv (Ty2_Ref (Rgn2_Const true true r) t0)) rgns /\ 
+                 included (free_rgn_vars_in_eps eff) rgns)
+      by (eapply IHHExp; eauto).
+    destruct H1 as [H2 H3].
+    intuition. inversion H.
+  - assert (H1 : included (frv (Ty2_Ref (Rgn2_Const true true r) t0)) rgns /\ 
+                 included (free_rgn_vars_in_eps eff) rgns)
+      by (eapply IHHExp; eauto).
+    destruct H1 as [H2 H3].
+    intuition. inversion H.
+  - assert (H1 : included (frv Ty2_Effect) rgns /\ 
+                 included (free_rgn_vars_in_eps eff1) rgns)
+      by (eapply IHHExp1; eauto).
+    assert (H2 : included (frv Ty2_Effect) rgns /\ 
+                 included (free_rgn_vars_in_eps eff2) rgns)
+      by (eapply IHHExp2; eauto).
+    destruct H1 as [H3 H4].
+    destruct H2 as [H5 H6].
+    split.
+    + do 2 intro. apply H3. assumption.
+    + intro. apply IncludedUnion_Static_Action_4; [apply H4 | apply H6].
+Qed.
+
+
+Theorem TcVal_implies_closed :
+  forall stty v t,
+    TcVal (stty, v, t) ->
+    (forall r, r # t).
+Proof.
+  intros stty v t HTcVal.
+  dependent induction HTcVal; intros;
+  try ( solve [ unfold not_set_elem, Complement; simpl;
+                intro; unfold Ensembles.In, empty_set in H; contradiction] ).
+  - unfold not_set_elem, Complement; simpl.
+    intro. destruct H1; [contradiction |contradict H1; apply H0].
+  - eapply TypedExpressionFrv in H2; eauto.  
+    eapply TcRhoIncludedNoFreeVars; eauto.
+    intuition.
+  - unfold not_set_elem, Complement; simpl. 
+    intro. destruct H; contradict H; [eapply IHHTcVal1 | eapply IHHTcVal2]; eauto.
+Qed.
+
+Lemma subst_rho_fresh_var :
+  forall rho rgns x stty v t r,
+    TcRho (rho, rgns) ->
+    not_set_elem rgns x ->
+    TcVal (stty, v, subst_rho rho t) ->
+    TcVal (stty, v, subst_rho rho (subst_in_type x r t)).
+Proof.
+  intros rho rgns x stty v t r HTcRho H_not_set HTcVal.
+  assert ( x # (subst_rho rho t)) by (eapply TcVal_implies_closed; eauto).
+  generalize dependent rgns.
+  generalize dependent r.
+  generalize dependent x.  
+  dependent induction HTcVal; intros;
+    inversion HTcRho as [rho' rgns' HRgn HVal'']; subst;
+  try (solve [ unfold subst_in_type;
+               assert (R.find (elt:=nat) x0 rho = None) 
+                 by (eapply contrapositiveTcRho; eauto; apply HRgn);
+               rewrite  SUBST_FRESH; [rewrite <- x; econstructor; eauto | 
+                                      eapply subst_rho_free_vars; eauto]  ] ).
+Qed.
+
+Lemma extended_rho : forall stty rho env ctxt,
+                       TcEnv (stty, rho, env, ctxt) ->
+                       forall x r rgns,
+                         TcRho (rho, rgns) ->
+                         not_set_elem rgns x -> 
+                         TcEnv (stty, update_R (x, r) rho, env, ctxt). 
+Proof.
+  intros stty rho env ctxt HEnv x r rgns HRho HRgns. 
+  inversion_clear HEnv as [ stty' rho' env' ctxt' ? HE HT HV]. 
+  inversion_clear HRho as [rho' rgns' HRgn' HVal''].
+  constructor; auto.
+  intros x0 v0 t0 HE' HT'. eapply HV in HE'; eauto. unfold update_R. simpl.
+  rewrite subst_add_comm. 
+  - eapply subst_rho_fresh_var; eauto. econstructor; auto. 
+  - unfold not_set_elem in HRgns. unfold Ensembles.Complement in HRgns.
+    intro. 
+    apply RMapP.in_find_iff in H0.
+    eapply HRgn' in H0. contradiction.
+Qed.
+
+
+Lemma TcRhoIncludedNoFreeVarsTyRef:
+  forall rho rgns r0 t x,
+    TcRho (rho, rgns) ->
+    included (set_union (free_rgn_vars_in_rgn r0) (frv t)) rgns ->
+    ~ free_rgn_vars_in_rgn (fold_subst_rgn rho r0) x.
+Proof.
+  intros rho rgns r0 t x HRho HInc H.
+  generalize dependent r0.
+  unfold Region_in_Type.
+  dependent induction r0; intros.
+  - rewrite subst_rho_rgn_const in H.
+    simpl in H. contradiction.
+  - destruct (AsciiVars.eq_dec x v) as [c | c].
+    + inversion c; subst.   
+      inversion HRho; subst.   
+      contradict H.
+      destruct (subst_rho_fvar_1 rho v) as [[v' H0] | H0]. 
+      * rewrite H0. simpl. intro. contradiction.
+      * rewrite H0. simpl. intro. 
+        unfold set_elem, In in H1.
+        destruct H1 with (r:=v). 
+        { apply H3 in HInc.
+          - apply NotNoneIsSome in HInc.
+            destruct HInc.
+            apply subst_rho_fvar_2 in H4.
+            rewrite H4 in H0. 
+            inversion H0.
+          - apply Union_introl. simpl. auto. }
+   + unfold AsciiVars.eq in c; subst.   
+     inversion HRho; subst.
+     contradict H.
+     destruct (subst_rho_fvar_1 rho v) as [[v' H0] | H0].
+     * rewrite H0. simpl. intro. contradiction.
+     * rewrite H0. simpl. intro. inversion H. auto.
+  - rewrite subst_rho_index in H.
+    simpl in H. contradiction. 
+Qed.
+
+
+
+Lemma TcRhoIncludedNoFreeVarsEps_main:
+  forall rho rgns e x,
+    TcRho (rho, rgns) ->
+    free_rgn_vars_in_eps e x ->
+    included (free_rgn_vars_in_eps e) rgns ->
+    ~ (free_rgn_vars_in_eps (fold_subst_eps rho e)) x.
+Proof.
+  intros.
+  apply TcRhoIncludedNoFreeVarsEps_find.
+  inversion H; subst. apply H3. apply H1.
+  unfold In.
+  assumption.
+Qed.
+
+Lemma TcRhoIncludedNoFreeVars:
+  forall rho rgns t r, 
+    TcRho (rho, rgns) ->
+    included (frv t) rgns ->
+    r # subst_rho rho t.
+Proof.
+  intros.
+  generalize dependent t.
+  dependent induction t; intro HInc; simpl in HInc.
+  - rewrite subst_rho_natural; simpl. intro. contradiction. 
+  - rewrite subst_rho_boolean; simpl. intro. contradiction.
+  - rewrite subst_rho_effect; simpl. intro. contradiction.
+  - rewrite subst_rho_unit; simpl. intro. contradiction.
+  - rewrite subst_rho_pair; simpl.
+    unfold not_set_elem, Complement. intro.
+    destruct H0.
+    + contradict H0. apply IHt1. 
+      unfold included, Included in *.
+      intros. apply HInc.
+      apply Ensembles.Union_introl.
+      assumption.
+    + contradict H0. apply IHt2. 
+      unfold included, Included in *.
+      intros. apply HInc.
+      apply Ensembles.Union_intror.
+      assumption.
+  - rewrite subst_rho_tyref; simpl. 
+    unfold not_set_elem, Complement. intro.
+    destruct H0.
+    + apply IHt.   
+      * unfold included, Included in *.
+        intros. apply HInc.
+        apply Ensembles.Union_intror.
+        assumption.
+      * contradict H0. unfold Ensembles.In.
+        eapply TcRhoIncludedNoFreeVarsTyRef; eauto.
+    + unfold included, Included, Ensembles.In in *.
+      apply IHt.
+      * intros. apply HInc. apply Ensembles.Union_intror. assumption.
+      * assumption.
+  - rewrite subst_rho_arrow; simpl.
+    unfold not_set_elem, Complement. intro.
+    destruct H0. 
+    + apply IHt1; auto. 
+      unfold included, Included in *. 
+      intros. apply HInc. apply Union_introl. assumption.
+    + destruct H0.
+      * { destruct H0.
+          - eapply TcRhoIncludedNoFreeVarsEps_main  with (e:=e); eauto.
+            + unfold In in H0. eapply TcRhoIncludedNoFreeVarsEps_aux_fold; eauto. 
+            + unfold included, Included, Ensembles.In in *.
+              intro. intro.
+              apply HInc.
+              apply Ensembles.Union_intror. apply Ensembles.Union_introl.
+              apply Ensembles.Union_introl. assumption.
+          - eapply TcRhoIncludedNoFreeVarsEps_main with (e:=e0); eauto.
+            + unfold In in H0. eapply TcRhoIncludedNoFreeVarsEps_aux_fold; eauto. 
+            + unfold included, Included, Ensembles.In in *.
+              intro. intro. apply HInc.
+              apply Ensembles.Union_intror. apply Ensembles.Union_introl.
+              apply Ensembles.Union_intror. assumption. }
+      * { repeat destruct H0.
+          - apply IHt2; auto. 
+            unfold included, Included in *. 
+            intros. apply HInc. 
+            apply Union_intror. apply Union_intror. apply Union_introl. assumption.
+          - apply IHt3; auto. 
+            unfold included, Included in *. 
+            intros. apply HInc. 
+            apply Union_intror. apply Union_intror. apply Union_intror. assumption. }
+  - rewrite subst_rho_forallrgn; simpl.
+    unfold not_set_elem, Complement. intro.
+    destruct H0.
+    + eapply TcRhoIncludedNoFreeVarsEps_main with (e:=e); eauto. 
+      * eapply TcRhoIncludedNoFreeVarsEps_aux_fold; eauto. 
+      * unfold included, Included, In in *. intro. intro.
+        apply HInc.
+        apply Union_introl. assumption.
+    + apply IHt; auto. 
+      unfold included, Included in *. 
+      intros. apply HInc. 
+      apply Union_intror. assumption.
+Qed.
+
+Lemma StoreTyping_Extended:
+  forall stty sttya sttyb,
+    (forall (l : ST.key) (t' : tau),
+       ST.find (elt:=tau) l stty = Some t' -> ST.find (elt:=tau) l sttya = Some t' ) ->
+    (forall (l : ST.key) (t' : tau),
+       ST.find (elt:=tau) l stty = Some t' -> ST.find (elt:=tau) l sttyb = Some t' ) ->
+    (forall (l : ST.key) (t' : tau),
+    	ST.find (elt:=tau) l stty = Some t' -> ST.find (elt:=tau) l (Functional_Map_Union sttya sttyb) = Some t' ).
+Proof. 
+  intros stty sttya sttyb Ha Hb.
+  intros l t' H.
+  edestruct (Ha l t' H).
+  generalize l. 
+  apply Functional_Map_Union_find.
+Qed.
+
+
+Lemma Raw_diff_key_1:
+  forall t a b v v' e,
+    Raw.bst e ->
+    b <> a ->
+    Raw.find (elt := t) a (Raw.add b v e) = Some v' -> 
+    Raw.find (elt := t) a e = Some v'.
+Proof.
+  intros. 
+  apply EProofs.find_1; auto.
+  apply EProofs.find_2 in H1. now apply EProofs.add_3 in H1.
+Qed.
+
+Require Import Lia.
+
+Lemma Raw_same_key:
+  forall t x v e, 
+    Raw.bst e ->
+    Raw.find (elt := t) x (Raw.add x v e) = Some v.
+Proof.
+  intros. rewrite EProofs.add_find; auto.
+  case_eq (AsciiVars.compare x x); intros; 
+  now try repeat (unfold AsciiVars.lt in l; lia).
+Qed.  
+
+Lemma Raw_diff_key_2:
+  forall t a b v v' e,
+    Raw.bst e ->
+    b <> a ->
+    Raw.find (elt := t) a e = Some v' ->
+    Raw.find (elt := t) a (Raw.add b v e) = Some v'.
+Proof.
+  intros. apply EProofs.find_1; 
+  [now apply EProofs.add_bst | apply EProofs.find_2 in H1; now apply EProofs.add_2 ].
+Qed.
+
+
+Lemma update_env:
+  forall stty rho env ctxt, 
+    TcEnv (stty, rho, env, ctxt) -> 
+    (forall x v t, 
+       TcVal (stty, v, subst_rho rho t) ->
+       TcEnv (stty, rho, update_E (x, v) env, update_T (x, t) ctxt) ).
+Proof. 
+  intros stty rho env ctxt HEnv x v t HTc.  
+  inversion_clear HEnv as [ stty' rho' env' ctxt' ? HE HT HV]. 
+  apply TC_Env;
+  unfold find_E, update_E, find_T, update_T in *; simpl.
+  clear HTc.
+  - now apply EProofs.add_bst. (** "env is a bst" **)
+  - intros x0 v0 HF. (** "TcEnv is well-typed: HE" **)
+    destruct (AsciiVars.eq_dec x0 x) as [c | c].
+    + unfold AsciiVars.eq in c; intros. 
+      subst. exists t. now rewrite E_same_key.
+    + unfold AsciiVars.eq in c; intros. 
+      eapply Raw_diff_key_1 in HF; auto; subst.
+      * destruct (HE x0 v0) as [t0 HU] ; [auto | ] ; exists t0.
+        eapply E_diff_key_2 ; [ auto | exact HU]. 
+  - intros x0 t0 HF. (** "TcEnv is well-typed: HT".  **)
+    destruct (AsciiVars.eq_dec x0 x) as [c | c]; 
+    unfold AsciiVars.eq in c; intros; subst.  
+    + exists v. now rewrite Raw_same_key.
+    + eapply E_diff_key_1 in HF; auto.
+      destruct (HT x0 t0) as [x1 ?] ; [auto | ].
+      exists x1; [eapply Raw_diff_key_2]; auto.
+  - intros x0 v0 t0 HFindE HFindT. (** "Type preservation: HV". **)
+    destruct (AsciiVars.eq_dec x0 x) as [c | c];
+    unfold AsciiVars.eq in c; intros; subst.
+    + rewrite Raw_same_key in HFindE by assumption.
+      inversion HFindE; subst.
+      rewrite E_same_key in HFindT by assumption.
+      inversion HFindT; subst. assumption.
+    + eapply Raw_diff_key_1 in HFindE; auto.
+      eapply E_diff_key_1 in HFindT; auto.
+      eapply HV; eauto.
+Qed.
